template-coq/theories/Universes.v
@@ -1,5 +1,6 @@
+From Coq Require Import ssreflect.
 From Coq Require Import MSetList MSetFacts MSetProperties MSetDecide.
-From MetaCoq.Template Require Import utils BasicAst config.
+From MetaCoq.Template Require Import utils BasicAst config Levels Sorts.
 
 Local Open Scope nat_scope.
 Local Open Scope string_scope2.
@@ -10,1213 +11,116 @@ Ltac absurd :=
   | [H : False |- _] => elim H
   end.
 Hint Extern 10 => absurd : core.
-(** * Valuations *)
-
-(** A valuation is a universe level (nat) given for each
-    universe variable (Level.t).
-    It is >= for polymorphic universes and > 0 for monomorphic universes. *)
-Record valuation :=
-  { valuation_mono : string -> positive ;
-    valuation_poly : nat -> nat }.
-
-Inductive universes :=
-  | UProp
-  | USProp
-  | UType (i : nat).
-
-Class Evaluable (A : Type) := val : valuation -> A -> nat.
-
-(** Levels are Set or Level or Var *)
-Module Level.
-  Inductive t_ : Set :=
-  | lSet
-  | Level (_ : string)
-  | Var (_ : nat) (* these are debruijn indices *).
-
-  Definition t := t_.
-
-  Definition is_small (x : t) :=
-    match x with
-    | lSet => true
-    | _ => false
-    end.
-
-  Definition is_set (x : t) :=
-    match x with
-    | lSet => true
-    | _ => false
-    end.
-
-  Definition is_var (l : t) :=
-    match l with
-    | Var _ => true
-    | _ => false
-    end.
-
-  Global Instance Evaluable : Evaluable t
-    := fun v l => match l with
-               | lSet =>  (0%nat)
-               | Level s => (Pos.to_nat (v.(valuation_mono) s))
-               | Var x => (v.(valuation_poly) x)
-               end.
-
-
-  Definition compare (l1 l2 : t) : comparison :=
-    match l1, l2 with
-    | lSet, lSet => Eq
-    | lSet, _ => Lt
-    | _, lSet => Gt
-    | Level s1, Level s2 => string_compare s1 s2
-    | Level _, _ => Lt
-    | _, Level _ => Gt
-    | Var n, Var m => Nat.compare n m
-    end.
-
-  Definition eq : t -> t -> Prop := eq.
-  Definition eq_equiv : Equivalence eq := _.
-
-  Definition eq_dec (l1 l2 : t) : {l1 = l2}+{l1 <> l2}.
-  Proof.
-    decide equality. apply string_dec. apply Peano_dec.eq_nat_dec.
-  Defined.
-
-  Inductive lt_ : t -> t -> Prop :=
-  | ltSetLevel s : lt_ lSet (Level s)
-  | ltSetVar n : lt_ lSet (Var n)
-  | ltLevelLevel s s' : string_lt s s' -> lt_ (Level s) (Level s')
-  | ltLevelVar s n : lt_ (Level s) (Var n)
-  | ltVarVar n n' : Nat.lt n n' -> lt_ (Var n) (Var n').
-
-  Definition lt := lt_.
-
-  Definition lt_strorder : StrictOrder lt.
-  Proof.
-    constructor.
-    - intros [| |] X; inversion X.
-      eapply string_lt_irreflexive; tea.
-      eapply Nat.lt_irrefl; tea.
-    - intros [| |] [| |] [| |] X1 X2;
-        inversion X1; inversion X2; constructor.
-      eapply transitive_string_lt; tea.
-      etransitivity; tea.
-  Qed.
-
-  Definition lt_compat : Proper (eq ==> eq ==> iff) lt.
-  Proof.
-    intros x y e z t e'. unfold eq in *; subst. reflexivity.
-  Qed.
-
-  Definition compare_spec :
-    forall x y : t, CompareSpec (x = y) (lt x y) (lt y x) (compare x y).
-  Proof.
-    intros [] []; repeat constructor.
-    - eapply CompareSpec_Proper.
-      5: eapply CompareSpec_string. 4: reflexivity.
-      all: split; [now inversion 1|]. now intros ->.
-      all: intro; now constructor.
-    - eapply CompareSpec_Proper.
-      5: eapply Nat.compare_spec. 4: reflexivity.
-      all: split; [now inversion 1|]. now intros ->.
-      all: intro; now constructor.
-  Qed.
-
-  (* Bonus *)
-  Definition eqb (l1 l2 : Level.t) : bool
-    := match compare l1 l2 with Eq => true | _ => false end.
-
-  Global Instance eqb_refl : Reflexive eqb.
-  Proof.
-    intros []; unfold eqb; cbnr.
-    - rewrite (ssreflect.iffRL (string_compare_eq s s)). all: auto.
-    - rewrite Nat.compare_refl. reflexivity.
-  Qed.
-
-  Lemma eqb_spec l l' : reflect (eq l l') (eqb l l').
-  Proof.
-    destruct l, l'; cbn; try constructor; try reflexivity; try discriminate.
-    - apply iff_reflect. unfold eqb; cbn.
-      destruct (CompareSpec_string s s0); split; intro HH;
-        try reflexivity; try discriminate; try congruence.
-      all: inversion HH; subst; now apply string_lt_irreflexive in H.
-    - apply iff_reflect. unfold eqb; cbn.
-      destruct (Nat.compare_spec n n0); split; intro HH;
-        try reflexivity; try discriminate; try congruence.
-      all: inversion HH; subst; now apply Nat.lt_irrefl in H.
-  Qed.
-
-  Definition eq_leibniz (x y : t) : eq x y -> x = y := id.
-
-End Level.
-
-Module LevelSet := MSetList.MakeWithLeibniz Level.
-Module LevelSetFact := WFactsOn Level LevelSet.
-Module LevelSetProp := WPropertiesOn Level LevelSet.
-Module LevelSetDecide := WDecide (LevelSet).
-Ltac lsets := LevelSetDecide.fsetdec.
-
-Definition LevelSet_pair x y
-  := LevelSet.add y (LevelSet.singleton x).
-
-Lemma LevelSet_pair_In x y z :
-  LevelSet.In x (LevelSet_pair y z) -> x = y \/ x = z.
-Proof.
-  intro H. apply LevelSetFact.add_iff in H.
-  destruct H; [intuition|].
-  apply LevelSetFact.singleton_1 in H; intuition.
-Qed.
-
-Definition LevelSet_mem_union (s s' : LevelSet.t) x :
-  LevelSet.mem x (LevelSet.union s s') <-> LevelSet.mem x s \/ LevelSet.mem x s'.
-Proof.
-  rewrite LevelSetFact.union_b.
-  apply orb_true_iff.
-Qed.
-
-
-(* prop level is Prop or SProp *)
-Module PropLevel.
-
-  Inductive t := lSProp | lProp.
-
-  (* Global Instance PropLevel_Evaluable : Evaluable t :=
-    fun v l => match l with
-              lSProp => -1
-            | lProp => -1
-            end. *)
-
-  Definition compare (l1 l2 : t) : comparison :=
-    match l1, l2 with
-    | lSProp, lSProp  => Eq
-    | lProp, lProp  => Eq
-    | lProp, lSProp => Gt
-    | lSProp, lProp => Lt
-    end.
-
-  Inductive lt_ : t -> t -> Prop :=
-    ltSPropProp : lt_ lSProp lProp.
-
-  Definition lt := lt_.
-
-  Global Instance lt_strorder : StrictOrder lt.
-  split.
-  - intros n X. destruct n;inversion X.
-  - intros n1 n2 n3 X1 X2. destruct n1,n2,n3;auto; try inversion X1;try inversion X2.
-  Defined.
-
-End PropLevel.
-
-Module UnivExpr.
-  (* npe = no prop expression *)
-  Definition t := (Level.t * nat)%type.
-
-  Global Instance Evaluable : Evaluable t
-    := fun v l => (snd l + val v (fst l)).
-
-  Definition succ (l : t) := (fst l, S (snd l)).
-
-  Definition get_level (e : t) : Level.t := fst e.
-
-  Definition get_noprop (e : UnivExpr.t) := Some (fst e).
-
-  Definition is_small (e : t) : bool :=
-    match e with
-    | (Level.lSet, 0%nat) => true
-    | _  => false
-    end.
-
-  Definition is_level (e : t) : bool :=
-    match e with
-    | (_, 0%nat) => true
-    | _  => false
-    end.
-
-  Definition make (l : Level.t) : t := (l, 0%nat).
-
-  Definition set : t := (Level.lSet, 0%nat).
-  Definition type1 : t := (Level.lSet, 1%nat).
-
-  (* Used for (un)quoting. *)
-  Definition from_kernel_repr (e : Level.t * bool) : t
-    := (e.1, if e.2 then 1%nat else 0%nat).
-
-  Definition to_kernel_repr (e : t) : Level.t * bool
-    := match e with
-       | (l, b) => (l, match b with 0%nat => false | _ => true end)
-       end.
-
-  Definition eq : t -> t -> Prop := eq.
-
-  Definition eq_equiv : Equivalence eq := _.
-
-  Inductive lt_ : t -> t -> Prop :=
-  | ltUnivExpr1 l n n' : (n < n')%nat -> lt_ (l, n) (l, n')
-  | ltUnivExpr2 l l' b b' : Level.lt l l' -> lt_ (l, b) (l', b').
-
-  Definition lt := lt_.
-
-  Global Instance lt_strorder : StrictOrder lt.
-  Proof.
-    constructor.
-    - intros x X; inversion X. subst. lia. subst.
-      eapply Level.lt_strorder; eassumption.
-    - intros x y z X1 X2; invs X1; invs X2; constructor; tea.
-      etransitivity; tea.
-      etransitivity; tea.
-  Qed.
-
-  Definition lt_compat : Proper (Logic.eq ==> Logic.eq ==> iff) lt.
-    intros x x' H1 y y' H2; now rewrite H1, H2.
-  Qed.
-
-  Definition compare (x y : t) : comparison :=
-    match x, y with
-    | (l1, b1), (l2, b2) =>
-      match Level.compare l1 l2 with
-      | Eq => Nat.compare b1 b2
-      | x => x
-      end
-    end.
-
-  Definition compare_spec :
-    forall x y : t, CompareSpec (x = y) (lt x y) (lt y x) (compare x y).
-  Proof.
-    intros [? ?] [? ?]; cbn; repeat constructor.
-    destruct (Level.compare_spec t0 t1); repeat constructor; tas.
-    subst. 
-    destruct (Nat.compare_spec n n0); repeat constructor; tas. congruence.
-  Qed.
-
-  Definition eq_dec (l1 l2 : t) : {l1 = l2} + {l1 <> l2}.
-  Proof.
-    repeat decide equality.
-  Defined.
-
-  Definition eq_leibniz (x y : t) : eq x y -> x = y := id.
-
-  Lemma val_make v l
-    : val v (UnivExpr.make l) = val v l.
-  Proof.
-    destruct l eqn:H; cbnr.
-  Qed.
-
-  Lemma val_make_npl v (l : Level.t)
-    : val v (UnivExpr.make l) = val v l.
-  Proof.
-    destruct l; cbnr.
-  Qed.
-
-End UnivExpr.
-
-Module UnivExprSet := MSetList.MakeWithLeibniz UnivExpr.
-Module UnivExprSetFact := WFactsOn UnivExpr UnivExprSet.
-Module UnivExprSetProp := WPropertiesOn UnivExpr UnivExprSet.
-
-Module Universe.
-  (** A universe is a list of universe expressions which is:
-        - sorted
-        - without duplicate
-        - non empty *)
-  Record t0 := { t_set : UnivExprSet.t ;
-                 t_ne  : UnivExprSet.is_empty t_set = false }.
-
-  Inductive t_ :=
-    lProp | lSProp | lType (_ : t0).
-
-  Definition t := t_.
-
-  Coercion t_set : t0 >-> UnivExprSet.t.
-
-  Definition eqb (u1 u2 : t) : bool :=
-    match u1, u2 with
-    | lSProp, lSProp => true
-    | lProp, lProp => true
-    | lType e1, lType e2 => UnivExprSet.equal e1.(t_set) e2.(t_set)
-    | _,_ => false
-    end.
-
-  Definition make' (e : UnivExpr.t) : t0
-    := {| t_set := UnivExprSet.singleton e;
-          t_ne := eq_refl |}.
-
-  (** Create a universe representing the given level. *)
-  Definition make (l : Level.t) : t :=
-    lType (make' (UnivExpr.make l)).
-
-  Definition of_expr e := (lType (make' e)).
-
-  Lemma not_Empty_is_empty s :
-    ~ UnivExprSet.Empty s -> UnivExprSet.is_empty s = false.
-  Proof.
-    intro H. apply not_true_is_false. intro H'.
-    apply H. now apply UnivExprSetFact.is_empty_2 in H'.
-  Qed.
-
-  Program Definition add (e : UnivExpr.t) (u : t0) : t0
-    := {| t_set := UnivExprSet.add e u |}.
-  Next Obligation.
-    apply not_Empty_is_empty; intro H.
-    eapply H. eapply UnivExprSet.add_spec.
-    left; reflexivity.
-  Qed.
-
-  Definition add_to_exprs (e : UnivExpr.t) (u : t) : t :=
-    match u with
-    | lSProp |lProp => u
-    | lType l => lType (add e l)
-    end.
-
-  Lemma add_spec e u e' :
-    UnivExprSet.In e' (add e u) <-> e' = e \/ UnivExprSet.In e' u.
-  Proof.
-    apply UnivExprSet.add_spec.
-  Qed.
-
-  Definition add_list : list UnivExpr.t -> t0 -> t0
-    := List.fold_left (fun u e => add e u).
-
-  Lemma add_list_spec l u e :
-    UnivExprSet.In e (add_list l u) <-> In e l \/ UnivExprSet.In e u.
-  Proof.
-    unfold add_list. rewrite <- fold_left_rev_right.
-    etransitivity. 2:{ eapply or_iff_compat_r. etransitivity.
-                       2: apply @InA_In_eq with (A:=UnivExpr.t).
-                       eapply InA_rev. }
-    induction (List.rev l); cbn.
-    - split. intuition. intros [H|H]; tas. invs H.
-    - split.
-      + intro H. apply add_spec in H. destruct H as [H|H].
-        * left. now constructor.
-        * apply IHl0 in H. destruct H as [H|H]; [left|now right].
-          now constructor 2.
-      + intros [H|H]. inv H.
-        * apply add_spec; now left.
-        * apply add_spec; right. apply IHl0. now left.
-        * apply add_spec; right. apply IHl0. now right.
-  Qed.
-
-  Definition add_list_to_exprs (es : list UnivExpr.t) (u : t) : t :=
-    match u with
-    | lSProp |lProp => u
-    | lType l => lType (add_list es l)
-    end.
-
-  (** Test if the universe is a lub of levels or contains +n's. *)
-  Definition is_levels (u : t) : bool :=
-      match u with
-      | lProp | lSProp => true
-      | lType l =>  UnivExprSet.for_all UnivExpr.is_level l
-      end.
-
-  (** Test if the universe is a level or an algebraic universe. *)
-  Definition is_level (u : t) : bool :=
-    match u with
-    | lProp | lSProp => true
-    | lType l => (UnivExprSet.cardinal l =? 1)%nat && is_levels u
-    end.
-
-  Definition is_small (u : t) : bool :=
-    match u with
-      | lProp | lSProp => true
-      | lType l => UnivExprSet.for_all UnivExpr.is_small l
-    end.
-
-  Definition is_sprop (u : t) : bool :=
-    match u with
-      | lSProp => true
-      | _ => false
-    end.
-
-  Definition is_prop (u : t) : bool :=
-    match u with
-      | lProp => true
-      | _ => false
-    end.
-
-  Definition type0 : t := make Level.lSet.
-  Definition type1 : t := lType (make' UnivExpr.type1).
-
-  Definition of_levels (l : PropLevel.t + Level.t) : t :=
-    match l with
-    | inl PropLevel.lSProp => lSProp
-    | inl PropLevel.lProp => lProp
-    | inr l => lType (make' (l, 0%nat))
-    end.
-
-  (* Used for quoting. *)
-  Definition from_kernel_repr (e : Level.t * bool) (es : list (Level.t * bool)) : t
-    := lType (add_list (map UnivExpr.from_kernel_repr es)
-                (make' (UnivExpr.from_kernel_repr e))).
-
-  (* Definition uex_to_kernel_repr (e : UnivExpr.t) : Level.t * bool := *)
-  (*   match e with *)
-  (*   | UnivExpr.npe (l, b) => (NoPropLevel.to_level l, b) *)
-  (*   end. *)
-
-  (* Definition to_kernel_repr (u : t) : list (Level.t * bool) *)
-  (*   :=  map (UnivExpr.to_kernel_repr) (UnivExprSet.elements u). *)
-  (* match u with *)
-  (*      | lProp => [(Level.lProp, false)] *)
-  (*      | lSProp => [(Level.lSProp, false)] *)
-  (*      | lType l => map uex_to_kernel_repr (UnivExprSet.elements l) *)
-  (*      end. *)
-
-
-  (** The non empty / sorted / without dup list of univ expressions, the
-      components of the pair are the head and the tail of the (non empty) list *)
-  Program Definition exprs (u : t0) : UnivExpr.t * list UnivExpr.t
-    := match UnivExprSet.elements u with
-       | [] => False_rect _ _
-       | e :: l => (e, l)
-       end.
-  Next Obligation.
-    destruct u as [u1 u2]; cbn in *. revert u2.
-    apply eq_true_false_abs.
-    unfold UnivExprSet.is_empty, UnivExprSet.Raw.is_empty,
-    UnivExprSet.elements, UnivExprSet.Raw.elements in *.
-    rewrite <- Heq_anonymous; reflexivity.
-  Qed.
-
-  Lemma exprs_make' e : Universe.exprs (Universe.make' e) = (e, []).
-  Proof. reflexivity. Defined.
-
-  (* Lemma exprs_make l : Universe.exprs (Universe.make l) = (UnivExpr.make l, []). *)
-  (* Proof. reflexivity. Defined. *)
-
-
-  Lemma exprs_spec u :
-    let '(e, u') := Universe.exprs u in
-    e :: u' = UnivExprSet.elements u.
-  Proof.
-    destruct u as [u1 u2].
-    pose (l := UnivExprSet.elements u1).
-    change (let '(e, u') :=
-                match l return l = UnivExprSet.elements u1 -> _ with
-                | [] => fun Heq_anonymous : [] = _ u1 =>
-                    False_rect (UnivExpr.t × list UnivExpr.t)
-                               (exprs_obligation_1
-                                  {| Universe.t_set := u1; Universe.t_ne := u2 |}
-                                  Heq_anonymous)
-                | e :: l0 => fun _ : e :: l0 = _ u1 => (e, l0)
-                end eq_refl in e :: u' = UnivExprSet.elements  u1).
-    set (e := eq_refl). clearbody e. change (l = UnivExprSet.elements u1) in e.
-    destruct l.
-    - exfalso. revert u2. apply eq_true_false_abs.
-      unfold UnivExprSet.is_empty, UnivExprSet.Raw.is_empty,
-      UnivExprSet.elements, UnivExprSet.Raw.elements in *.
-      rewrite <- e; reflexivity.
-    - assumption.
-  Qed.
-
-  Lemma exprs_spec' u :
-    (Universe.exprs u).1 :: (Universe.exprs u).2 = UnivExprSet.elements u.
-  Proof.
-    pose proof (exprs_spec u).
-    now destruct (Universe.exprs u).
-  Qed.
-
-  Lemma In_exprs (u : t0) (e : UnivExpr.t) :
-    UnivExprSet.In e u
-    <-> e = (Universe.exprs u).1 \/ In e (Universe.exprs u).2.
-  Proof.
-    etransitivity. symmetry. apply UnivExprSet.elements_spec1.
-    pose proof (Universe.exprs_spec' u) as H.
-    destruct (Universe.exprs u) as [e' l]; cbn in *.
-    rewrite <- H; clear. etransitivity. apply InA_cons.
-    eapply or_iff_compat_l. apply InA_In_eq.
-  Qed.
-
-  Lemma In_exprs_rev (u : t0) (e : UnivExpr.t) :
-    UnivExprSet.In e u
-    <-> e = (Universe.exprs u).1 \/ In e (List.rev (Universe.exprs u).2).
-  Proof.
-    etransitivity. eapply In_exprs.
-    apply or_iff_compat_l. apply in_rev.
-  Qed.
-
-  Definition map (f : UnivExpr.t -> UnivExpr.t) (u : t0) : t0 :=
-    let '(e, l) := exprs u in
-    add_list (List.map f l) (make' (f e)).
-
-  Lemma map_spec f u e :
-    UnivExprSet.In e (map f u) <-> exists e0, UnivExprSet.In e0 u /\ e = (f e0).
-  Proof.
-    unfold map. symmetry. etransitivity.
-    { eapply iff_ex; intro. eapply and_iff_compat_r. eapply In_exprs. }
-    destruct (exprs u) as [e' l]; cbn in *.
-    symmetry. etransitivity. eapply add_list_spec.
-    etransitivity. eapply or_iff_compat_l. apply UnivExprSet.singleton_spec.
-    etransitivity. eapply or_iff_compat_r.
-    apply in_map_iff. clear u. split.
-    - intros [[e0 []]|H].
-      + exists e0. split. right; tas. congruence.
-      + exists e'. split; tas. left; reflexivity.
-    - intros [xx [[H|H] ?]].
-      + right. congruence.
-      + left. exists xx. split; tas; congruence.
-  Qed.
-
-  (** The universe strictly above FOR TYPING (not cumulativity) *)
-
-  Definition super (l : t) : t :=
-    match l with
-    | lSProp => type1
-    | lProp => type1
-    | lType l => lType (map UnivExpr.succ l)
-    end.
-
-  (** The l.u.b. of 2 non-prop universe sets *)
-  Program Definition sup0 (u v : t0) : t0 :=
-    {| t_set := UnivExprSet.union u v |}.
-  Next Obligation.
-    apply not_Empty_is_empty; intro H.
-    assert (HH: UnivExprSet.Empty u). {
-      intros x Hx. apply (H x).
-      eapply UnivExprSet.union_spec. now left. }
-    apply UnivExprSetFact.is_empty_1 in HH.
-    rewrite t_ne in HH; discriminate.
-  Qed.
-
-  Definition sup (u v : t) : t :=
-    match u,v with
-    | lSProp, lProp => lProp
-    | lProp, lSProp => lProp
-    | (lSProp | lProp), u' => u'
-    | u', (lSProp | lProp) => u'
-    | lType l1, lType l2  => lType (sup0 l1 l2)
-    end.
-
-  Definition get_univ_exprs (u : t) (H1 : is_prop u = false) (H2 : is_sprop u = false) : t0.
-  destruct u; try discriminate;easy. Defined.
-
-  (** Type of a product *)
-  Definition sort_of_product (domsort rangsort : t) :=
-    (* Prop and SProp impredicativity *)
-    if Universe.is_prop rangsort || Universe.is_sprop rangsort then rangsort
-    else Universe.sup domsort rangsort.
-
-  Lemma eqb_refl u : eqb u u.
-  Proof.
-    destruct u;auto.
-    now apply UnivExprSet.equal_spec.
-  Qed.
-
-  Lemma elements_not_empty (u : Universe.t0) : UnivExprSet.elements u <> [].
-  Proof.
-    destruct u as [u1 u2]; cbn; intro e.
-    unfold UnivExprSet.is_empty, UnivExprSet.elements,
-    UnivExprSet.Raw.elements in *.
-    rewrite e in u2; discriminate.
-  Qed.
-
-  Definition get_is_level (u : t) : option Level.t :=
-    match u with
-    | lSProp => None
-    | lProp => None
-    | lType l => match UnivExprSet.elements l with
-                 [(l, 0%nat)] => Some l
-               | _ => None
-               end
-    end.
-
-  Global Instance Evaluable' : Evaluable t0
-    := fun v u => let '(e, u) := Universe.exprs u in
-               List.fold_left (fun n e => Nat.max (val v e) n) u (val v e).
-
-  Definition univ_val :=
-    fun v u => match u with
-            | lSProp => USProp
-            | lProp => UProp
-            | lType l => UType (val v l)
-            end.
-
-  Lemma val_make' v e
-    : val v (make' e) = val v e.
-  Proof.
-    reflexivity.
-  Qed.
-
-  Lemma val_make v l
-    : univ_val v (make l) = UType (val v l).
-  Proof.
-    destruct l; cbnr.
-  Qed.
-
-  Lemma val_make_npl v (l : Level.t)
-    : univ_val v (make l) = UType (val v l).
-  Proof.
-    destruct l; cbnr.
-  Qed.
-
-  Lemma make_inj x y :
-    make x = make y -> x = y.
-  Proof.
-    destruct x, y; try now inversion 1.
-  Qed.
-
-End Universe.
-
-Definition is_propositional u := 
-  Universe.is_prop u || Universe.is_sprop u.
-
-(** This coercion allows to see the universes as a [UnivExprSet.t] *)
-Coercion Universe.t_set : Universe.t0 >-> UnivExprSet.t.
-
-Declare Scope univ_scope.
-Delimit Scope univ_scope with u.
-
-Notation "⟦ u ⟧_ v" := (Universe.univ_val v u) (at level 0, format "⟦ u ⟧_ v", v ident) : univ_scope.
-
-Ltac u :=
- change LevelSet.elt with Level.t in *;
- change UnivExprSet.elt with UnivExpr.t in *.
- (* change ConstraintSet.elt with UnivConstraint.t in *. *)
-
-
-Lemma val_fold_right (u : Universe.t0) v :
-  val v u = fold_right (fun e x => Nat.max (val v e) x) (val v (Universe.exprs u).1)
-                       (List.rev (Universe.exprs u).2).
-Proof.
-  unfold val at 1, Universe.Evaluable'.
-  destruct (Universe.exprs u).
-  now rewrite fold_left_rev_right.
-Qed.
-
-Lemma val_In_le (u : Universe.t0) v e :
-  UnivExprSet.In e u -> val v e <= val v u.
-Proof.
-  intro H. rewrite val_fold_right.
-  apply Universe.In_exprs_rev in H. destruct (Universe.exprs u); cbn in *.
-  clear -H. destruct H as [H|H].
-  - subst. induction (List.rev l); cbnr; lia.
-  - induction (List.rev l); cbn; invs H.
-    + u; lia.
-    + specialize (IHl0 H0). lia.
-Qed.
-
-Lemma val_In_max (u : Universe.t0) v :
-  exists e, UnivExprSet.In e u /\ val v e = val v u.
-Proof.
-  eapply iff_ex. {
-    intro. eapply and_iff_compat_r. apply Universe.In_exprs_rev. }
-  rewrite val_fold_right. destruct (Universe.exprs u) as [e l]; cbn in *.
-  clear. induction (List.rev l); cbn.
-  - exists e. split; cbnr. left; reflexivity.
-  - destruct IHl0 as [e' [H1 H2]].
-    destruct (Nat.max_dec (val v a) (fold_right (fun e0 x0 => Nat.max (val v e0) x0)
-                                               (val v e) l0)) as [H|H];
-      rewrite H; clear H.
-    + exists a. split; cbnr. right. now constructor.
-    + rewrite <- H2. exists e'. split; cbnr.
-      destruct H1 as [H1|H1]; [now left|right]. now constructor 2.
-Qed.
-
-Lemma val_ge_caract (u : Universe.t0) v k :
-  (forall e, UnivExprSet.In e u -> val v e <= k) <-> val v u <= k.
-Proof.
-  split.
-  - eapply imp_iff_compat_r. {
-      eapply iff_forall; intro. eapply imp_iff_compat_r.
-      apply Universe.In_exprs_rev. }
-    rewrite val_fold_right.
-    destruct (Universe.exprs u) as [e l]; cbn; clear.
-    induction (List.rev l); cbn.
-    + intros H. apply H. left; reflexivity.
-    + intros H.
-      destruct (Nat.max_dec (val v a) (fold_right (fun e0 x => Nat.max (val v e0) x)
-                                                 (val v e) l0)) as [H'|H'];
-        rewrite H'; clear H'.
-      * apply H. right. now constructor.
-      * apply IHl0. intros x [H0|H0]; apply H. now left.
-        right; now constructor 2.
-  - intros H e He. eapply val_In_le in He. etransitivity; eassumption.
-Qed.
-
-Lemma val_le_caract (u : Universe.t0) v k :
-  (exists e, UnivExprSet.In e u /\ k <= val v e) <-> k <= val v u.
-Proof.
-  split.
-  - eapply imp_iff_compat_r. {
-      eapply iff_ex; intro. eapply and_iff_compat_r. apply Universe.In_exprs_rev. }
-    rewrite val_fold_right.
-    destruct (Universe.exprs u) as [e l]; cbn; clear.
-    induction (List.rev l); cbn.
-    + intros H. destruct H as [e' [[H1|H1] H2]].
-      * now subst.
-      * invs H1.
-    + intros [e' [[H1|H1] H2]].
-      * forward IHl0; [|lia]. exists e'. split; tas. left; assumption.
-      * invs H1.
-        -- u; lia.
-        -- forward IHl0; [|lia]. exists e'. split; tas. right; assumption.
-  - intros H. destruct (val_In_max u v) as [e [H1 H2]].
-    exists e. rewrite H2; split; assumption.
-Qed.
-
-
-
-Lemma val_caract (u : Universe.t0) v k :
-  val v u = k
-  <-> (forall e, UnivExprSet.In e u -> val v e <= k)
-    /\ exists e, UnivExprSet.In e u /\ val v e = k.
-Proof.
-  split.
-  - intros <-; split.
-    + apply val_In_le.
-    + apply val_In_max.
-  - intros [H1 H2].
-    apply val_ge_caract in H1.
-    assert (k <= val v u); [clear H1|lia].
-    apply val_le_caract. destruct H2 as [e [H2 H2']].
-    exists e. split; tas. lia.
-Qed.
-
-Lemma val_add v e s
-  : val v (Universe.add e s) = Nat.max (val v e) (val v s).
-Proof.
-  apply val_caract. split.
-  - intros e' H. apply UnivExprSet.add_spec in H. destruct H as [H|H].
-    + subst. u; lia.
-    + eapply val_In_le with (v:=v) in H. lia.
-  - destruct (Nat.max_dec (val v e) (val v s)) as [H|H]; rewrite H; clear H.
-    + exists e. split; cbnr. apply UnivExprSetFact.add_1. reflexivity.
-    + destruct (val_In_max s v) as [e' [H1 H2]].
-      exists e'. split; tas. now apply UnivExprSetFact.add_2.
-Qed.
-
-Lemma val_sup v s1 s2 :
-  val v (Universe.sup0 s1 s2) = Nat.max (val v s1) (val v s2).
-Proof.
-  eapply val_caract. cbn. split.
-  - intros e' H. eapply UnivExprSet.union_spec in H. destruct H as [H|H].
-    + eapply val_In_le with (v:=v) in H. lia.
-    + eapply val_In_le with (v:=v) in H. lia.
-  - destruct (Nat.max_dec (val v s1) (val v s2)) as [H|H]; rewrite H; clear H.
-    + destruct (val_In_max s1 v) as [e' [H1 H2]].
-      exists e'. split; tas. apply UnivExprSet.union_spec. now left.
-    + destruct (val_In_max s2 v) as [e' [H1 H2]].
-      exists e'. split; tas. apply UnivExprSet.union_spec. now right.
-Qed.
-
-Ltac proper := let H := fresh in try (intros ? ? H; destruct H; reflexivity).
-
-Lemma for_all_elements (P : UnivExpr.t -> bool) u :
-  UnivExprSet.for_all P u = forallb P (UnivExprSet.elements u).
-Proof.
-  apply UnivExprSetFact.for_all_b; proper.
-Qed.
-
-Definition univ_val_max v1 v2 :=
-  match v1, v2 with
-  | UProp, UProp => UProp
-  | USProp, USProp => USProp
-  | UType v, UType v' => UType (Nat.max v v')
-  | _, UType _ => v2
-  | UType _, _ => v1
-  | UProp, USProp => UProp
-  | USProp, UProp => UProp
-  end.
-
-Lemma val_universe_sup v u1 u2 :
-  Universe.univ_val v (Universe.sup u1 u2) = univ_val_max (Universe.univ_val v u1) (Universe.univ_val v u2).
-Proof.
-  destruct u1 as [ | | l1]; destruct u2 as [ | | l2];cbn;try lia; auto.
-  f_equal. apply val_sup.
-Qed.
-
-Lemma is_prop_val u :
-  Universe.is_prop u -> forall v, Universe.univ_val v u = UProp.
-Proof.
-  destruct u as [| | u];try discriminate;auto.
-Qed.
-
-Lemma is_sprop_val u :
-  Universe.is_sprop u -> forall v, Universe.univ_val v u = USProp.
-Proof.
-  destruct u as [| | u];try discriminate;auto.
-Qed.
-
-(* 
-Lemma val_zero_exprs v (l : Universe.t0) : 0 <= val v l.
-Proof.
-  rewrite val_fold_right.
-  destruct (Universe.exprs l) as [e u']; clear l; cbn.
-  induction (List.rev u'); simpl.
-  - destruct e as [npl_expr].
-    destruct npl_expr as [t b].
-    cbn.
-    assert (0 <= val v t) by apply Level.val_zero.
-    destruct b;lia.
-  - pose proof (UnivExpr.val_zero a v); lia.
-Qed. *)
-
-
-Lemma val_is_prop u v :
-  Universe.univ_val v u = UProp <-> Universe.is_prop u.
-Proof.
-  destruct u; auto;cbn in *; intuition congruence.
-Qed.
-
-Lemma val_is_sprop u v :
-  Universe.univ_val v u = USProp <-> Universe.is_sprop u.
-Proof.
-  destruct u;auto;cbn in *; intuition congruence.
-Qed.
-
-Lemma is_prop_and_is_sprop_val_false u :
-  Universe.is_prop u = false -> Universe.is_sprop u = false -> 
-  forall v, ∑ n, Universe.univ_val v u = UType n.
-Proof.
-  intros Hp Hsp v.
-  destruct u; try discriminate. simpl. eexists; eauto.
-Qed.
-
-Lemma val_is_prop_false u v n :
-  Universe.univ_val v u = UType n -> Universe.is_prop u = false.
-Proof.
-  pose proof (is_prop_val u) as H. destruct (Universe.is_prop u); cbnr.
-  rewrite (H eq_refl v). discriminate.
-Qed.
-
-Lemma eq_univ (u v : Universe.t0) :
-  u = v :> UnivExprSet.t -> u = v.
-Proof.
-  destruct u as [u1 u2], v as [v1 v2]; cbn. intros X; destruct X.
-  now rewrite (uip_bool _ _ u2 v2).
-Qed.
-
-Lemma eq_univ' (u v : Universe.t0) :
-  UnivExprSet.Equal u v -> u = v.
-Proof.
-  intro H. now apply eq_univ, UnivExprSet.eq_leibniz.
-Qed.
-
-Lemma eq_univ'' (u v : Universe.t0) :
-  UnivExprSet.elements u = UnivExprSet.elements v -> u = v.
-Proof.
-  intro H. apply eq_univ.
-  destruct u as [u1 u2], v as [v1 v2]; cbn in *; clear u2 v2.
-  destruct u1 as [u1 u2], v1 as [v1 v2]; cbn in *.
-  destruct H. now rewrite (uip_bool _ _ u2 v2).
-Qed.
-
-Lemma get_is_level_correct u l :
-  Universe.get_is_level u = Some l -> u = Universe.make l.
-Proof.
-  intro H.
-  destruct u eqn:Hu;cbn in *.
-  - inversion H;subst;reflexivity.
-  - inversion H;subst;reflexivity.
-  - unfold Universe.make.
-    destruct (UnivExprSet.elements _) as [|l0 L] eqn:Hu1; [discriminate|].
-    destruct l0, L; try discriminate.
-    * destruct t,n;inversion H;subst.
-      apply f_equal.
-      apply eq_univ'';unfold UnivExpr.make.
-      cbn. simpl in Hu1. rewrite Hu1. reflexivity.
-    * destruct e,n;inversion H;subst.
-Qed.
-
-Lemma univ_expr_eqb_true_iff (u v : Universe.t0) :
-  UnivExprSet.equal u v <-> u = v.
-Proof.
-  split.
-  - intros.
-    apply eq_univ'. now apply UnivExprSet.equal_spec.
-  - intros ->. now apply UnivExprSet.equal_spec.
-Qed.
-
-Lemma eqb_true_iff u v :
-  Universe.eqb u v <-> u = v.
-Proof.
-  split. 2: intros ->; apply Universe.eqb_refl.
-  intro H.
-  destruct u,v;auto;try discriminate.
-  apply f_equal. now apply univ_expr_eqb_true_iff.
-Qed.
-
-Lemma UnivExprSet_for_all_false f u :
-  UnivExprSet.for_all f u = false -> UnivExprSet.exists_ (negb ∘ f) u.
-Proof.
-  intro H. rewrite UnivExprSetFact.exists_b.
-  rewrite UnivExprSetFact.for_all_b in H.
-  all: try now intros x y [].
-  induction (UnivExprSet.elements u); cbn in *; [discriminate|].
-  apply andb_false_iff in H; apply orb_true_iff; destruct H as [H|H].
-  left; now rewrite H.
-  right; now rewrite IHl.
-Qed.
-
-Lemma UnivExprSet_For_all_exprs (P : UnivExpr.t -> Prop) (u : Universe.t0)
-  : UnivExprSet.For_all P u
-    <-> P (Universe.exprs u).1 /\ Forall P (Universe.exprs u).2.
-Proof.
-  etransitivity.
-  - eapply iff_forall; intro e. eapply imp_iff_compat_r.
-    apply Universe.In_exprs.
-  - cbn; split.
-    + intro H. split. apply H. now left.
-      apply Forall_forall. intros x H0.  apply H; now right.
-    + intros [H1 H2] e [He|He]. subst e; tas.
-      eapply Forall_forall in H2; tea.
-Qed.
-
-Lemma sup0_comm x1 x2 :
-  Universe.sup0 x1 x2 = Universe.sup0 x2 x1.
-Proof.
-  apply eq_univ'; simpl. unfold UnivExprSet.Equal.
-  intros H. rewrite !UnivExprSet.union_spec. intuition.
-Qed.
-
-Lemma sup_comm x1 x2 :
-  Universe.sup x1 x2 = Universe.sup x2 x1.
-Proof.
-  destruct x1,x2;auto.
-  cbn;apply f_equal;apply sup0_comm.
-Qed.
-
-Lemma is_prop_sort_sup x1 x2 :
-  Universe.is_prop (Universe.sup x1 x2)
-  -> Universe.is_prop x2 \/ Universe.is_sprop x2 .
-Proof. destruct x1,x2;auto. Qed.
-
-Lemma is_prop_sort_sup' x1 x2 :
-  Universe.is_prop (Universe.sup x1 x2)
-  -> Universe.is_prop x1 \/ Universe.is_sprop x1 .
-Proof. destruct x1,x2;auto. Qed.
-
-Lemma is_prop_or_sprop_sort_sup x1 x2 :
-  Universe.is_sprop (Universe.sup x1 x2) -> Universe.is_sprop x2.
-Proof. destruct x1,x2;auto. Qed.
-
-Lemma is_prop_sort_sup_prop x1 x2 :
-  Universe.is_prop x1 && Universe.is_prop x2 ->
-  Universe.is_prop (Universe.sup x1 x2).
-Proof. destruct x1,x2;auto. Qed.
-
-Lemma is_prop_or_sprop_sort_sup_prop x1 x2 :
-  Universe.is_sprop x1 && Universe.is_sprop x2 ->
-  Universe.is_sprop (Universe.sup x1 x2).
-Proof. destruct x1,x2;auto. Qed.
-
-Lemma is_prop_sup u s :
-  Universe.is_prop (Universe.sup u s) ->
-  (Universe.is_prop u \/ Universe.is_sprop u) /\
-  (Universe.is_prop s \/ Universe.is_sprop s).
-Proof. destruct u,s;auto. Qed.
-
-Lemma is_sprop_sup_iff u s :
-  Universe.is_sprop (Universe.sup u s) <->
-  (Universe.is_sprop u /\ Universe.is_sprop s).
-Proof. split;destruct u,s;intuition. Qed.
-
-Lemma is_prop_sort_prod x2 x3 :
-  Universe.is_prop (Universe.sort_of_product x2 x3)
-  -> Universe.is_prop x3.
-Proof.
-  unfold Universe.sort_of_product.
-  destruct x3;cbn;auto.
-  intros;simpl in *;destruct x2;auto.
-Qed.
-
-Lemma is_sprop_sort_prod x2 x3 :
-  Universe.is_sprop (Universe.sort_of_product x2 x3)
-  -> Universe.is_sprop x3.
-Proof.
-  unfold Universe.sort_of_product.
-  destruct x3;cbn;auto.
-  intros;simpl in *;destruct x2;auto.
-Qed.
-
-(** Sort families *)
-
-Inductive sort_family : Set := InSProp | InProp | InSet | InType.
-
-(* Prop <= Set, Type but SProp </= Prop, Set, Type *)
-Definition leb_sort_family x y :=
-  match x, y with
-  | InProp, InSProp => false
-  | InProp, _ => true
-  | InSProp, InSProp => true
-  | InSProp, _ => false
-  | InSet, (InProp | InSProp) => false
-  | InSet, _ => true
-  | InType, (InProp | InSProp | InSet) => false
-  | InType, InType => true
-  end.
-
-(** Family of a universe [u]. *)
-Definition universe_family (u : Universe.t) :=
-  if Universe.is_prop u then InProp
-  else if Universe.is_sprop u then InSProp
-  else if Universe.is_small u then InSet
-  else InType.
-
-Module ConstraintType.
-  Inductive t_ : Set := Le (z : Z) | Eq.
-  Definition t := t_.
-  Definition eq : t -> t -> Prop := eq.
-  Definition eq_equiv : Equivalence eq := _.
-
-  Definition Le0 := Le 0.
-  Definition Lt := Le 1.
-
-  Inductive lt_ : t -> t -> Prop :=
-  | LeLe n m : (n < m)%Z -> lt_ (Le n) (Le m)
-  | LeEq n : lt_ (Le n) Eq.
-  Definition lt := lt_.
-
-  Lemma lt_strorder : StrictOrder lt.
-  Proof.
-    constructor.
-    - intros []; intro X; inversion X. lia.
-    - intros ? ? ? X Y; invs X; invs Y; constructor. lia.
-  Qed.
-
-  Lemma lt_compat : Proper (eq ==> eq ==> iff) lt.
-  Proof.
-    intros ? ? X ? ? Y; invs X; invs Y. reflexivity.
-  Qed.
-
-  Definition compare (x y : t) : comparison :=
-    match x, y with
-    | Le n, Le m => Z.compare n m
-    | Le _, Eq => Datatypes.Lt
-    | Eq, Eq => Datatypes.Eq
-    | Eq, _  => Datatypes.Gt
-    end.
-
-  Lemma compare_spec x y : CompareSpec (eq x y) (lt x y) (lt y x) (compare x y).
-  Proof.
-    destruct x, y; repeat constructor. simpl.
-    destruct (Z.compare_spec z z0); simpl; constructor.
-    subst; constructor. now constructor. now constructor.
-  Qed.
-
-  Lemma eq_dec x y : {eq x y} + {~ eq x y}.
-  Proof.
-    unfold eq. decide equality.
-    apply Z.eq_dec.
-  Qed.
-End ConstraintType.
-
-Module UnivConstraint.
-  Definition t : Set := Level.t * ConstraintType.t * Level.t.
-  Definition eq : t -> t -> Prop := eq.
-  Definition eq_equiv : Equivalence eq := _.
-
-  Definition make l1 ct l2 : t := (l1, ct, l2).
-
-  Inductive lt_ : t -> t -> Prop :=
-  | lt_Level2 l1 t l2 l2' : Level.lt l2 l2' -> lt_ (l1, t, l2) (l1, t, l2')
-  | lt_Cstr l1 t t' l2 l2' : ConstraintType.lt t t' -> lt_ (l1, t, l2) (l1, t', l2')
-  | lt_Level1 l1 l1' t t' l2 l2' : Level.lt l1 l1' -> lt_ (l1, t, l2) (l1', t', l2').
-  Definition lt := lt_.
-
-  Lemma lt_strorder : StrictOrder lt.
-  Proof.
-    constructor.
-    - intros []; intro X; inversion X; subst;
-        try (eapply Level.lt_strorder; eassumption).
-      eapply ConstraintType.lt_strorder; eassumption.
-    - intros ? ? ? X Y; invs X; invs Y; constructor; tea.
-      etransitivity; eassumption.
-      2: etransitivity; eassumption.
-      eapply ConstraintType.lt_strorder; eassumption.
-  Qed.
-
-  Lemma lt_compat : Proper (eq ==> eq ==> iff) lt.
-  Proof.
-    intros ? ? X ? ? Y; invs X; invs Y. reflexivity.
-  Qed.
-
-  Definition compare : t -> t -> comparison :=
-    fun '(l1, t, l2) '(l1', t', l2') =>
-      Pos.switch_Eq (Pos.switch_Eq (Level.compare l2 l2')
-                                   (ConstraintType.compare t t'))
-                    (Level.compare l1 l1').
-
-  Lemma compare_spec x y
-    : CompareSpec (eq x y) (lt x y) (lt y x) (compare x y).
-  Proof.
-    destruct x as [[l1 t] l2], y as [[l1' t'] l2']; cbn.
-    destruct (Level.compare_spec l1 l1'); cbn; repeat constructor; tas.
-    invs H.
-    destruct (ConstraintType.compare_spec t t'); cbn; repeat constructor; tas.
-    invs H.
-    destruct (Level.compare_spec l2 l2'); cbn; repeat constructor; tas.
-    invs H. reflexivity.
-  Qed.
-
-  Lemma eq_dec x y : {eq x y} + {~ eq x y}.
-  Proof.
-    unfold eq. repeat decide equality.
-  Defined.
-
-  Definition eq_leibniz (x y : t) : eq x y -> x = y := id.
-End UnivConstraint.
-
-Module ConstraintSet := MSetList.MakeWithLeibniz UnivConstraint.
-Module ConstraintSetFact := WFactsOn UnivConstraint ConstraintSet.
-Module ConstraintSetProp := WPropertiesOn UnivConstraint ConstraintSet.
-
 
 (** {6 Universe instances} *)
 
 Module Instance.
 
-  (** A universe instance represents a vector of argument universes
-      to a polymorphic definition (constant, inductive or constructor). *)
-  Definition t : Set := list Level.t.
+  (** A universe instance represents a vector of argument sorts
+      to a polymorphic definition (constant, inductive or constructor).
+      The optional level needs to be present if the sort is predicative. *)
+  Definition t : Set := list Level.t * list SortFamily.t.
 
-  Definition empty : t := [].
+  Definition empty : t := ([], []).
   Definition is_empty (i : t) : bool :=
     match i with
-    | [] => true
+    | ([], []) => true
     | _ => false
     end.
 
   Definition eqb (i j : t) :=
-    forallb2 Level.eqb i j.
+    forallb2 Level.eqb (fst i) (fst j) && forallb2 SortFamily.eqb (snd i) (snd j).
 
   Definition equal_upto (f : Level.t -> Level.t -> bool) (i j : t) :=
-    forallb2 f i j.
+    forallb2 f (fst i) (fst j) && forallb2 SortFamily.eqb (snd i) (snd j).
 End Instance.
 
+Module ConstraintSet.
+  Definition t := SortConstraintFormula.t × UnivConstraintSet.t.
 
+  Definition empty := (SortConstraintFormula.True, UnivConstraintSet.empty).
 
+  Definition is_empty t :=
+    SortConstraintFormula.is_True (fst t) && UnivConstraintSet.is_empty (snd t).
+End ConstraintSet.
+
+(** ** Contexts *)
+
+(** * Universe Context *)
+(* Context of named variables *)
 Module UContext.
   Definition t := Instance.t × ConstraintSet.t.
 
-  Definition make : Instance.t -> ConstraintSet.t -> t := pair.
+  Definition make : Instance.t -> SortConstraintFormula.t -> UnivConstraintSet.t -> t :=
+    fun ins scs ucs => (ins, (scs, ucs)).
 
-  Definition empty : t := (Instance.empty, ConstraintSet.empty).
+  Definition empty : t :=
+    (Instance.empty, ConstraintSet.empty).
 
   Definition instance : t -> Instance.t := fst.
-  Definition constraints : t -> ConstraintSet.t := snd.
+  Definition sort_constraints : t -> SortConstraintFormula.t := fst ∘ snd.
+  Definition univ_constraints : t -> UnivConstraintSet.t := snd ∘ snd.
 
-  Definition dest : t -> Instance.t * ConstraintSet.t := fun x => x.
+  Definition dest : t -> Instance.t * (SortConstraintFormula.t * UnivConstraintSet.t) := fun x => x.
 End UContext.
 
-Module AUContext.
-  Definition t := list name × ConstraintSet.t.
 
-  Definition make (ids : list name) (ctrs : ConstraintSet.t) : t := (ids, ctrs).
+(** * Abstract Universe Context *)
+(* Context of DeBruijn variables *)
+Module AUContext.
+
+  (* Following the convention of Instance.t
+     the first list is for universe-levels, the second for sort families
+     names are irrelevant *)
+  Definition t := (list name × list name) × ConstraintSet.t.
+
+  Definition make (lvl_ids sort_ids: list name) (sctrs : SortConstraintFormula.t) (uctrs : UnivConstraintSet.t) : t := ((lvl_ids, sort_ids), (sctrs, uctrs)).
+
   Definition repr (x : t) : UContext.t :=
-    let (u, cst) := x in
-    (mapi (fun i _ => Level.Var i) u, cst).
+    let '((uvs0,sorts0), cst) := x in
+    let uvs := mapi (fun i _ => Level.Var i) uvs0 in
+    let sorts := mapi (fun i _ => SortFamily.sfVar i) sorts0 in
+    ((uvs, sorts), cst).
 
   Definition levels (uctx : t) : LevelSet.t :=
-    LevelSetProp.of_list (fst (repr uctx)).
+    LevelSetProp.of_list (fst (fst (repr uctx))).
 End AUContext.
 
-Module ContextSet.
-  Definition t := LevelSet.t × ConstraintSet.t.
+(** * Only for monomorphic universes *)
+Module UnivContextSet.
+  Definition t := LevelSet.t × UnivConstraintSet.t.
 
-  Definition empty : t := (LevelSet.empty, ConstraintSet.empty).
+  Definition empty : t := (LevelSet.empty, UnivConstraintSet.empty).
 
   Definition is_empty (uctx : t)
-    := LevelSet.is_empty (fst uctx) && ConstraintSet.is_empty (snd uctx).
-End ContextSet.
+    := LevelSet.is_empty (fst uctx) && UnivConstraintSet.is_empty (snd uctx).
+End UnivContextSet.
+
+
+Inductive universes_decl : Type :=
+| Monomorphic_ctx (ctx : UnivContextSet.t)
+| Polymorphic_ctx (cst : AUContext.t).
+
+Definition monomorphic_udecl u :=
+  match u with
+  | Monomorphic_ctx ctx => ctx
+  | _ => UnivContextSet.empty
+  end.
+
+Definition monomorphic_levels φ := (monomorphic_udecl φ).1.
+Definition monomorphic_constraints φ := (monomorphic_udecl φ).2.
+
+Definition levels_of_udecl u :=
+  match u with
+  | Monomorphic_ctx ctx => fst ctx
+  | Polymorphic_ctx ctx => AUContext.levels ctx
+  end.
+
+Definition universe_constraints_of_udecl u :=
+  match u with
+  | Monomorphic_ctx ctx => snd ctx
+  | Polymorphic_ctx ctx => snd (snd (AUContext.repr ctx))
+  end.
 
 
 (* Variance info is needed to do full universe polymorphism *)
@@ -1234,67 +138,22 @@ Module Variance.
   (* val sup : t -> t -> t *)
 End Variance.
 
-Inductive universes_decl : Type :=
-| Monomorphic_ctx (ctx : ContextSet.t)
-| Polymorphic_ctx (cst : AUContext.t).
 
-Definition monomorphic_udecl u :=
-  match u with
-  | Monomorphic_ctx ctx => ctx
-  | _ => ContextSet.empty
-  end.
-
-Definition monomorphic_levels φ := (monomorphic_udecl φ).1.
-Definition monomorphic_constraints φ := (monomorphic_udecl φ).2.
-
-Definition levels_of_udecl u :=
-  match u with
-  | Monomorphic_ctx ctx => fst ctx
-  | Polymorphic_ctx ctx => AUContext.levels ctx
-  end.
-
-Definition constraints_of_udecl u :=
-  match u with
-  | Monomorphic_ctx ctx => snd ctx
-  | Polymorphic_ctx ctx => snd (AUContext.repr ctx)
-  end.
-
-Definition univ_le_n {cf:checker_flags} n u u' := 
-  match u, u' with
-  | UProp, UProp
-  | USProp, USProp => (n = 0)%Z
-  | UType u, UType u' => (Z.of_nat u <= Z.of_nat u' - n)%Z
-  | UProp, UType u => 
-    if prop_sub_type then True else False
-  | _, _ => False
-  end.
+Definition univ_le_n n u u' :=
+  (Z.of_nat u <= Z.of_nat u' - n)%Z.
 
 Notation "x <_ n y" := (univ_le_n n x y) (at level 10, n ident) : univ_scope.
 Notation "x < y" := (univ_le_n 1 x y) : univ_scope.
 Notation "x <= y" := (univ_le_n 0 x y) : univ_scope.
 
 Ltac lle := unfold univ_le_n in *.
-Ltac lled := lle; match goal with
-                  | H : prop_sub_type = true |- _ => rewrite H in *
-                  | H : prop_sub_type = false |- _ => rewrite H in *
-                  | H : is_true prop_sub_type |- _ => rewrite H in *
-                  | _ => destruct prop_sub_type eqn:?Hb
-                  end.
-
-Ltac prop_non_prop :=
-  match goal with
-  | |- context[ Universe.is_prop ?u || Universe.is_sprop ?u]  =>
-    destruct (Universe.is_prop u || Universe.is_sprop u)
-  | H : context[ Universe.is_prop ?u || Universe.is_sprop ?u] |- _ =>
-    destruct (Universe.is_prop u || Universe.is_sprop u)
-  end.
 
 Section Univ.
   Context {cf:checker_flags}.
 
   Global Instance lle_refl : Reflexive (univ_le_n 0).
   Proof.
-    intro x. destruct x; simpl; lia.
+    intro x; red; lia.
   Qed.
 
   Lemma switch_minus (x y z : Z) : (x <= y - z <-> x + z <= y)%Z.
@@ -1303,7 +162,7 @@ Section Univ.
 
   Global Instance le_n_trans n : Transitive (univ_le_n (Z.of_nat n)).
   Proof.
-    intros [] [] []; unfold univ_le_n; simpl; try lia; try (destruct prop_sub_type; lia).
+    intros ? ? ?; unfold univ_le_n; simpl; lia.
   Qed.
 
   Global Instance lle_trans : Transitive (univ_le_n 0).
@@ -1312,46 +171,27 @@ Section Univ.
   Global Instance llt_trans : Transitive (univ_le_n 1).
   Proof. apply (le_n_trans 1). Qed.
 
-  (* Lemma llt_lt n m : (n < m)%u -> (n < m)%Z.
-  Proof. lled; lia. Qed.
-
-  Lemma lle_le n m : (n <= m)%u -> (n <= m)%Z.
-  Proof. lled; lia. Qed.
-
-  Lemma lt_llt n m : prop_sub_type -> (n < m)%Z -> (n < m)%u.
-  Proof. unfold llt. now intros ->. Qed.
-
-  Lemma le_lle n m : prop_sub_type -> (n <= m)%Z -> (n <= m)%u.
-  Proof. lled; [lia|discriminate]. Qed.
-
-  Lemma lt_llt' n m : (0 <= n)%Z -> (n < m)%Z -> (n < m)%u.
-  Proof. lled; lia. Qed.
-
-  Lemma le_lle' n m : (0 <= n)%Z -> (n <= m)%Z -> (n <= m)%u.
-  Proof. lled; lia. Qed. *)
-
-
   Inductive satisfies0 (v : valuation) : UnivConstraint.t -> Prop :=
   | satisfies0_Lt (l l' : Level.t) (z : Z) : (Z.of_nat (val v l) <= Z.of_nat (val v l') - z)%Z
-                         -> satisfies0 v (l, ConstraintType.Le z, l')
+                         -> satisfies0 v (l, UnivConstraintType.Le z, l')
   | satisfies0_Eq (l l' : Level.t) : val v l = val v l'
-                         -> satisfies0 v (l, ConstraintType.Eq, l').
+                         -> satisfies0 v (l, UnivConstraintType.Eq, l').
 
-  Definition satisfies v : ConstraintSet.t -> Prop :=
-    ConstraintSet.For_all (satisfies0 v).
+  Definition satisfies v : UnivConstraintSet.t -> Prop :=
+    UnivConstraintSet.For_all (satisfies0 v).
 
   Definition consistent ctrs := exists v, satisfies v ctrs.
 
-  Definition eq_universe0 (φ : ConstraintSet.t) u u' :=
-    forall v, satisfies v φ -> (Universe.univ_val v u = Universe.univ_val v u').
+  Definition eq_universe0 (φ : UnivConstraintSet.t) u u' :=
+    forall v, satisfies v φ -> (val v u = val v u').
 
-  Definition leq_universe_n n (φ : ConstraintSet.t) u u' :=
-    forall v, satisfies v φ -> (univ_le_n n (Universe.univ_val v u) (Universe.univ_val v u'))%u.
+  Definition leq_universe_n n (φ : UnivConstraintSet.t) u u' :=
+    forall v, satisfies v φ -> (univ_le_n n (val v u) (val v u'))%u.
 
-  Definition leq_universe0 (φ : ConstraintSet.t) u u' :=
-    forall v, satisfies v φ -> (Universe.univ_val v u <= Universe.univ_val v u')%u.
+  Definition leq_universe0 (φ : UnivConstraintSet.t) u u' :=
+    forall v, satisfies v φ -> (val v u <= val v u')%u.
 
-  Lemma leq_universe0_leq_universe_n (φ : ConstraintSet.t) u u' :
+  Lemma leq_universe0_leq_universe_n (φ : UnivConstraintSet.t) u u' :
     leq_universe0 φ u u' <-> leq_universe_n 0 φ u u'.
   Proof. intros. reflexivity. Qed.
 
@@ -1372,7 +212,7 @@ Section Univ.
     := if check_univs then valid_constraints0 φ ctrs else True.
 
   Lemma valid_subset φ φ' ctrs
-    : ConstraintSet.Subset φ φ' -> valid_constraints φ ctrs
+    : UnivConstraintSet.Subset φ φ' -> valid_constraints φ ctrs
       ->  valid_constraints φ' ctrs.
   Proof.
     unfold valid_constraints.
@@ -1455,51 +295,36 @@ Section Univ.
     intro H; split; intros v Hv; specialize (H v Hv); now rewrite H.
     intros [H1 H2] v Hv; specialize (H1 v Hv); specialize (H2 v Hv).
     unfold univ_le_n in *.
-    destruct (Universe.univ_val v u), (Universe.univ_val v u'); try now auto.
+    destruct (val v u), (val v u'); try now auto.
   Qed.
 
-  Lemma leq_universe0_sup_l φ s1 s2 :
-    Universe.is_prop s1 = false -> Universe.is_sprop s1 = false -> 
-    leq_universe0 φ s1 (Universe.sup s1 s2).
+
+  Lemma leq_universe0_sup_l' φ (s1 s2 : UniverseLevel.t) :
+    leq_universe0 φ s1 (UniverseLevel.sup s1 s2).
   Proof.
-    intros H1 H2 v Hv.
-    specialize (is_prop_and_is_sprop_val_false _ H1 H2 v) as [n Hzero].
-    rewrite val_universe_sup, Hzero. destruct (Universe.univ_val v s2); simpl; lia.
+    intros v Hv. cbn. rewrite val_sup. red; lia.
   Qed.
 
-  Lemma leq_universe0_sup_r φ s1 s2 :
-    Universe.is_prop s2 = false -> Universe.is_sprop s2 = false -> 
-    leq_universe0 φ s2 (Universe.sup s1 s2).
+  Lemma leq_universe0_sup_r' φ (s1 s2 : UniverseLevel.t) :
+    leq_universe0 φ s2 (UniverseLevel.sup s1 s2).
   Proof.
-    intros H1 H2 v Hv.
-    specialize (is_prop_and_is_sprop_val_false _ H1 H2 v) as [n Hzero].
-    rewrite val_universe_sup, Hzero.
-    destruct (Universe.univ_val v s1); simpl; lia.
+    intros v Hv. cbn. rewrite val_sup. red; lia.
   Qed.
 
-  Lemma leq_universe0_sup_l' φ (s1 s2 : Universe.t0) :
-    leq_universe0 φ (Universe.lType s1) (Universe.lType (Universe.sup0 s1 s2)).
-  Proof.
-    intros v Hv. cbn. rewrite val_sup. lia.
-  Qed.
-
-  Lemma leq_universe0_sup_r' φ (s1 s2 : Universe.t0) :
-    leq_universe0 φ (Universe.lType s2) (Universe.lType (Universe.sup0 s1 s2)).
-  Proof.
-    intros v Hv. cbn. rewrite val_sup. lia.
-  Qed.
-
-  Lemma leq_universe_product φ (s1 s2 : Universe.t)
-    : leq_universe φ s2 (Universe.sort_of_product s1 s2).
+  Lemma leq_universe_product φ (s1 s2 : UniverseLevel.t)
+    : leq_universe φ s2 (UniverseLevel.level_of_product s1 s2).
   Proof.
     unfold leq_universe; destruct check_univs; [cbn|constructor].
-    unfold Universe.sort_of_product.
-    destruct s2; cbn; try apply leq_universe0_refl.
-    destruct s1;cbn;try apply leq_universe0_refl.
     apply leq_universe0_sup_r'.
   Qed.
-  (* Rk: [leq_universe φ s1 (sort_of_product s1 s2)] does not hold due to
-     impredicativity. *)
+
+  (* We are only comparing universe levels for predicative sorts *)
+  Lemma leq_universe_product_dom φ (s1 s2 : UniverseLevel.t)
+    : leq_universe φ s1 (UniverseLevel.level_of_product s1 s2).
+  Proof.
+    unfold leq_universe; destruct check_univs; [cbn|constructor].
+    apply leq_universe0_sup_l'.
+  Qed.
 
   Global Instance eq_universe_leq_universe φ : subrelation (eq_universe φ) (leq_universe φ).
   Proof.
@@ -1524,15 +349,14 @@ Section Univ.
   Global Instance llt_str_order : StrictOrder (univ_le_n 1).
   Proof.
     split.
-    - intros x H. destruct x; simpl in *; lia.
+    - intros x H. red in H. simpl in *; lia.
     - exact _.
   Qed.
 
 
   Global Instance lle_antisym : Antisymmetric _ eq (univ_le_n 0).
   Proof.
-    intros [] []; simpl; try reflexivity; auto.
-    intros. f_equal; lia.
+    intros ? ? h h'; red in h, h'; lia.
   Qed.
 
   Global Instance leq_universe0_antisym φ
@@ -1573,10 +397,142 @@ Section Univ.
 End Univ.
 
 
-(* This universe is a hack used in plugings to generate fresh universes *)
-Definition fresh_universe : Universe.t. exact Universe.type0. Qed.
-(* This level is a hack used in plugings to generate fresh levels *)
-Definition fresh_level : Level.t. exact Level.lSet. Qed.
+
+
+
+(* (** * NOT SURE IF RELEVANT *) *)
+
+(* Inductive universes := *)
+(*   | UProp *)
+(*   | USProp *)
+(*   | UType (i : nat). *)
+
+(* Definition univ_val := *)
+(*   fun v u => match u with *)
+(*           | lSProp => USProp *)
+(*           | lProp => UProp *)
+(*           | lType l => UType (val v l) *)
+(*           end. *)
+
+
+(* Lemma val_make v l *)
+(*   : univ_val v (make l) = UType (val v l). *)
+(* Proof. *)
+(*   destruct l; cbnr. *)
+(* Qed. *)
+
+(* Lemma val_make_npl v (l : Level.t) *)
+(*   : univ_val v (make l) = UType (val v l). *)
+(* Proof. *)
+(*   destruct l; cbnr. *)
+(* Qed. *)
+
+
+(* Definition is_propositional u :=  *)
+(*   Universe.is_prop u || Universe.is_sprop u. *)
+
+(* (** This coercion allows to see the universes as a [UnivExprSet.t] *) *)
+(* Coercion Universe.t_set : Universe.t0 >-> UnivExprSet.t. *)
+
+(* Notation "⟦ u ⟧_ v" := (Universe.univ_val v u) (at level 0, format "⟦ u ⟧_ v", v ident) : univ_scope. *)
+
+
+(* (* Definition univ_val_max v1 v2 := *) *)
+(* (*   match v1, v2 with *) *)
+(* (*   | UProp, UProp => UProp *) *)
+(* (*   | USProp, USProp => USProp *) *)
+(* (*   | UType v, UType v' => UType (Nat.max v v') *) *)
+(* (*   | _, UType _ => v2 *) *)
+(* (*   | UType _, _ => v1 *) *)
+(* (*   | UProp, USProp => UProp *) *)
+(* (*   | USProp, UProp => UProp *) *)
+(* (*   end. *) *)
+
+(* (* Lemma val_universe_sup v u1 u2 : *) *)
+(* (*   Universe.univ_val v (Universe.sup u1 u2) = univ_val_max (Universe.univ_val v u1) (Universe.univ_val v u2). *) *)
+(* (* Proof. *) *)
+(* (*   destruct u1 as [ | | l1]; destruct u2 as [ | | l2];cbn;try lia; auto. *) *)
+(* (*   f_equal. apply val_sup. *) *)
+(* (* Qed. *) *)
+
+(* (* Lemma is_prop_val u : *) *)
+(* (*   Universe.is_prop u -> forall v, Universe.univ_val v u = UProp. *) *)
+(* (* Proof. *) *)
+(* (*   destruct u as [| | u];try discriminate;auto. *) *)
+(* (* Qed. *) *)
+
+(* (* Lemma is_sprop_val u : *) *)
+(* (*   Universe.is_sprop u -> forall v, Universe.univ_val v u = USProp. *) *)
+(* (* Proof. *) *)
+(* (*   destruct u as [| | u];try discriminate;auto. *) *)
+(* (* Qed. *) *)
+
+
+(* (* Lemma val_is_prop u v : *) *)
+(* (*   Universe.univ_val v u = UProp <-> Universe.is_prop u. *) *)
+(* (* Proof. *) *)
+(* (*   destruct u; auto;cbn in *; intuition congruence. *) *)
+(* (* Qed. *) *)
+
+(* (* Lemma val_is_sprop u v : *) *)
+(* (*   Universe.univ_val v u = USProp <-> Universe.is_sprop u. *) *)
+(* (* Proof. *) *)
+(* (*   destruct u;auto;cbn in *; intuition congruence. *) *)
+(* (* Qed. *) *)
+
+(* (* Lemma is_prop_and_is_sprop_val_false u : *) *)
+(* (*   Universe.is_prop u = false -> Universe.is_sprop u = false ->  *) *)
+(* (*   forall v, ∑ n, Universe.univ_val v u = UType n. *) *)
+(* (* Proof. *) *)
+(* (*   intros Hp Hsp v. *) *)
+(* (*   destruct u; try discriminate. simpl. eexists; eauto. *) *)
+(* (* Qed. *) *)
+
+(* (* Lemma val_is_prop_false u v n : *) *)
+(* (*   Universe.univ_val v u = UType n -> Universe.is_prop u = false. *) *)
+(* (* Proof. *) *)
+(* (*   pose proof (is_prop_val u) as H. destruct (Universe.is_prop u); cbnr. *) *)
+(* (*   rewrite (H eq_refl v). discriminate. *) *)
+(* (* Qed. *) *)
+
+
+
+(* (** Sort families *) *)
+
+(* Inductive sort_family : Set := InSProp | InProp | InSet | InType. *)
+
+(* (* Prop <= Set, Type but SProp </= Prop, Set, Type *) *)
+(* Definition leb_sort_family x y := *)
+(*   match x, y with *)
+(*   | InProp, InSProp => false *)
+(*   | InProp, _ => true *)
+(*   | InSProp, InSProp => true *)
+(*   | InSProp, _ => false *)
+(*   | InSet, (InProp | InSProp) => false *)
+(*   | InSet, _ => true *)
+(*   | InType, (InProp | InSProp | InSet) => false *)
+(*   | InType, InType => true *)
+(*   end. *)
+
+(* (** Family of a universe [u]. *) *)
+(* Definition universe_family (u : Universe.t) := *)
+(*   if Universe.is_prop u then InProp *)
+(*   else if Universe.is_sprop u then InSProp *)
+(*   else if Universe.is_small u then InSet *)
+(*   else InType. *)
+
+(* (** * END NOT SURE IF RELEVANT *) *)
+
+
+
+
+
+(* This universe is a hack used in plugins to generate fresh universes *)
+Definition fresh_universe : UniverseLevel.t.
+Proof. exact UniverseLevel.type0. Qed.
+(* This level is a hack used in plugins to generate fresh levels *)
+Definition fresh_level : Level.t.
+Proof. exact Level.lSet. Qed.
 
 
 (** * Universe substitution
@@ -1589,46 +545,80 @@ Definition fresh_level : Level.t. exact Level.lSet. Qed.
 
 Class UnivSubst A := subst_instance : Instance.t -> A -> A.
 
-
 Instance subst_instance_level : UnivSubst Level.t :=
-  fun u l => match l with
-            Level.lSet | Level.Level _ => l
-          | Level.Var n => List.nth n u Level.lSet
-          end.
+  fun u l =>
+    match l with
+    | Level.lSet | Level.Level _ => l
+    | Level.Var n => List.nth n (fst u) Level.lSet
+    end.
 
-Instance subst_instance_cstr : UnivSubst UnivConstraint.t :=
+Instance subst_instance_sort_family : UnivSubst SortFamily.t :=
+  fun u sf =>
+    match sf with
+    | SortFamily.sfType | SortFamily.sfGlobal _ => sf
+    | SortFamily.sfVar i => List.nth i (snd u) SortFamily.sfType
+    end.
+
+Instance subst_instance_ucstr : UnivSubst UnivConstraint.t :=
   fun u c => (subst_instance_level u c.1.1, c.1.2, subst_instance_level u c.2).
 
+Instance subst_instance_scstr : UnivSubst SortConstraint.t :=
+  fun u '(SortConstraint.Eliminable sf1 sf2) =>
+    SortConstraint.Eliminable (subst_instance u sf1) (subst_instance u sf2).
+
+Instance subst_instance_clause : UnivSubst SortConstraintSet.t :=
+  fun u ctrs =>
+    SortConstraintSet.fold
+      (fun c => SortConstraintSet.add (subst_instance_scstr u c))
+      ctrs SortConstraintSet.empty.
+
+Instance subst_instance_formula : UnivSubst SortConstraintFormula.t :=
+  fun u ctrs =>
+    SortConstraintFormula.fold
+      (fun c => SortConstraintFormula.add (subst_instance u c))
+      ctrs SortConstraintFormula.empty.
+
+Instance subst_instance_ucstrs : UnivSubst UnivConstraintSet.t :=
+  fun u ctrs =>
+    UnivConstraintSet.fold
+      (fun c => UnivConstraintSet.add (subst_instance u c))
+      ctrs UnivConstraintSet.empty.
+
 Instance subst_instance_cstrs : UnivSubst ConstraintSet.t :=
-  fun u ctrs => ConstraintSet.fold (fun c => ConstraintSet.add (subst_instance_cstr u c))
-                                ctrs ConstraintSet.empty.
+  fun u ctrs => (subst_instance u (fst ctrs), subst_instance u (snd ctrs)).
 
 Instance subst_instance_level_expr : UnivSubst UnivExpr.t :=
   fun u e => match e with
           | (Level.lSet, _)
           | (Level.Level _, _) => e
           | (Level.Var n, b) =>
-            match nth_error u n with
+            match nth_error (fst u) n with
             | Some l => (l,b)
             | None => (Level.lSet, b)
             end
           end.
 
-Instance subst_instance_univ0 : UnivSubst Universe.t0 :=
-  fun u => Universe.map (subst_instance_level_expr u).
+Instance subst_instance_univ_level : UnivSubst UniverseLevel.t :=
+  fun u => UniverseLevel.map (subst_instance_level_expr u).
 
-Instance subst_instance_univ : UnivSubst Universe.t :=
-  fun u e => match e with
-          | Universe.lProp | Universe.lSProp => e
-          | Universe.lType l => Universe.lType (subst_instance u l)
-          end.
+Instance subst_instance_sort : UnivSubst Sort.t :=
+  fun u s =>
+    match s with
+    | Sort.ImpredicativeSort sf =>
+      Sort.ImpredicativeSort (subst_instance u sf)
+    | Sort.PredicativeSort sf l =>
+      Sort.PredicativeSort (subst_instance u sf) (subst_instance u l)
+    end.
 
 Instance subst_instance_instance : UnivSubst Instance.t :=
-  fun u u' => List.map (subst_instance_level u) u'.
+  fun u u' =>
+    (List.map (subst_instance_level u) (fst u'),
+     List.map (subst_instance_sort_family u) (snd u')).
 
-(** Tests that the term is closed over [k] universe variables *)
+
+(** Tests that the term is closed over [j] sort variables and [k] universe level variables *)
 Section Closedu.
-  Context (k : nat).
+  Context (j k : nat).
 
   Definition closedu_level (l : Level.t) :=
     match l with
@@ -1639,17 +629,26 @@ Section Closedu.
   Definition closedu_level_expr (s : UnivExpr.t) :=
     closedu_level (UnivExpr.get_level s).
 
-  Definition closedu_universe_levels (u : Universe.t0) :=
+  Definition closedu_universe_levels (u : UniverseLevel.t) :=
     UnivExprSet.for_all closedu_level_expr u.
 
-  Definition closedu_universe (u : Universe.t) :=
+  Definition closedu_sort_family (sf : SortFamily.t) :=
+    match sf with
+    | SortFamily.sfVar i => (i <? j)%nat
+    | _ => true
+    end.
+
+  Definition closedu_universe (u : Sort.t) :=
     match u with
-    | Universe.lSProp | Universe.lProp => true
-    | Universe.lType l => closedu_universe_levels l
+    | Sort.ImpredicativeSort sf => closedu_sort_family sf
+    | Sort.PredicativeSort sf l =>
+      closedu_sort_family sf &&
+      closedu_universe_levels l
     end.
 
   Definition closedu_instance (u : Instance.t) :=
-    forallb closedu_level u.
+    forallb closedu_level (fst u)
+    && forallb closedu_sort_family (snd u).
 End Closedu.
 
 (** Universe-closed terms are unaffected by universe substitution. *)
@@ -1667,89 +666,134 @@ Section UniverseClosedSubst.
     destruct e as [t b]. destruct t;cbnr. discriminate.
   Qed.
 
-  Lemma closedu_subst_instance_univ u s
-    : closedu_universe 0 s -> subst_instance_univ u s = s.
+  Lemma closedu_subst_instance_univ_levels u s
+    : closedu_universe_levels 0 s -> subst_instance_univ_level u s = s.
   Proof.
-    intro H.
-    destruct s;auto;cbn in *.
-    apply f_equal. apply eq_univ'.
-    destruct t as [ts H1].
+    intros H; destruct s as [elts Hs].
+    unfold closedu_universe_levels in *;cbn in *.
+    unfold subst_instance_univ_level. simpl.
+    apply eq_univ'.
     unfold closedu_universe_levels in *;cbn in *.
     intro e; split; intro He.
-    - apply Universe.map_spec in He. destruct He as [e' [He' X]].
+    - apply UniverseLevel.map_spec in He. destruct He as [e' [He' X]].
       rewrite closedu_subst_instance_level_expr in X.
-      now subst. apply UnivExprSet.for_all_spec in H; proper.
+      2: now subst.
+      apply UnivExprSet.for_all_spec in H; proper.
       exact (H _ He').
-    - apply Universe.map_spec. exists e; split; tas.
+    - apply UniverseLevel.map_spec. exists e; split; tas.
       symmetry; apply closedu_subst_instance_level_expr.
       apply UnivExprSet.for_all_spec in H; proper. now apply H.
   Qed.
 
-  Lemma closedu_subst_instance_instance u t
-    : closedu_instance 0 t -> subst_instance_instance u t = t.
+
+  Lemma closedu_subst_instance_sort_family u sf
+    : closedu_sort_family 0 sf -> subst_instance_sort_family u sf = sf.
+  Proof. intros; destruct sf; cbnr; discriminate. Qed.
+
+  Lemma closedu_subst_instance_sort u s
+    : closedu_universe 0 0 s -> subst_instance_sort u s = s.
   Proof.
-    intro H. apply forall_map_id_spec.
-    apply Forall_forall; intros l Hl.
-    apply closedu_subst_instance_level.
-    eapply forallb_forall in H; eassumption.
+    intro H.
+    destruct s;auto;cbn in *; f_equal.
+    - move: H => /andP [+ _]; apply closedu_subst_instance_sort_family.
+    - move: H => /andP [_]; apply closedu_subst_instance_univ_levels.
+    - now apply closedu_subst_instance_sort_family.
+  Qed.
+
+  Lemma closedu_subst_instance_instance u t
+    : closedu_instance 0 0 t -> subst_instance_instance u t = t.
+  Proof.
+    intros [H1 H2]%andP.
+    destruct t as [t1 t2].
+    unfold subst_instance_instance; f_equal.
+    all: apply forall_map_id_spec; apply Forall_forall; intros l Hl.
+    1: {
+      apply closedu_subst_instance_level.
+      eapply forallb_forall in H1; eassumption.
+    }
+    apply closedu_subst_instance_sort_family.
+    eapply forallb_forall in H2; eassumption.
   Qed.
 
 End UniverseClosedSubst.
 
 Hint Resolve closedu_subst_instance_level closedu_subst_instance_level_expr
-     closedu_subst_instance_univ closedu_subst_instance_instance : substu.
+     closedu_subst_instance_univ_levels closedu_subst_instance_sort_family
+     closedu_subst_instance_sort closedu_subst_instance_instance : substu.
 
 (** Substitution of a universe-closed instance of the right size
     produces a universe-closed term. *)
 Section SubstInstanceClosed.
-  Context (u : Instance.t) (Hcl : closedu_instance 0 u).
+  Context (u : Instance.t) (Hcl : closedu_instance 0 0 u).
 
   Lemma subst_instance_level_closedu l
-    : closedu_level #|u| l -> closedu_level 0 (subst_instance_level u l).
+    : closedu_level #|fst u| l -> closedu_level 0 (subst_instance_level u l).
   Proof.
-    destruct l; cbnr.
-    unfold closedu_instance in Hcl.
-    destruct (nth_in_or_default n u Level.lSet).
-    - intros _. eapply forallb_forall in Hcl; tea.
+    destruct l; cbnr; move: Hcl=> /andP [H1 _].
+    destruct (nth_in_or_default n (fst u) Level.lSet).
+    - intros _. eapply forallb_forall in H1; tea.
     - rewrite e; reflexivity.
   Qed.
 
   Lemma subst_instance_level_expr_closedu e :
-    closedu_level_expr #|u| e -> closedu_level_expr 0 (subst_instance_level_expr u e).
+    closedu_level_expr #|fst u| e -> closedu_level_expr 0 (subst_instance_level_expr u e).
   Proof.
-    destruct e as [l b]. destruct l;cbnr.
-    case_eq (nth_error u n); cbnr. intros [] Hl X; cbnr.
+    destruct e as [l b]. destruct l;cbnr; move: Hcl=> /andP [H1 _].
+    case_eq (nth_error (fst u) n); cbnr. intros [] Hl X; cbnr.
     apply nth_error_In in Hl.
-    eapply forallb_forall in Hcl; tea.
+    eapply forallb_forall in H1; tea.
     discriminate.
   Qed.
 
-  Lemma subst_instance_univ_closedu s
-    : closedu_universe #|u| s -> closedu_universe 0 (subst_instance_univ u s).
+  Lemma subst_instance_universe_levels_closedu s
+    : closedu_universe_levels #|fst u| s -> closedu_universe_levels 0 (subst_instance u s).
   Proof.
     intro H.
-    destruct s;cbnr.
-    destruct t as [l Hl].
+    destruct s as [l Hl];cbnr.
     apply UnivExprSet.for_all_spec; proper.
-    intros e He. eapply Universe.map_spec in He.
+    intros e He. eapply UniverseLevel.map_spec in He.
     destruct He as [e' [He' X]]; subst.
     apply subst_instance_level_expr_closedu.
     apply UnivExprSet.for_all_spec in H; proper.
     now apply H.
   Qed.
 
-  Lemma subst_instance_instance_closedu t :
-    closedu_instance #|u| t -> closedu_instance 0 (subst_instance_instance u t).
+  Lemma subst_instance_sort_family_closedu sf :
+    closedu_sort_family #|snd u| sf -> closedu_sort_family 0 (subst_instance_sort_family u sf).
   Proof.
-    intro H. etransitivity. eapply forallb_map.
-    eapply forallb_impl; tea.
-    intros l Hl; cbn. apply subst_instance_level_closedu.
+    intro H; destruct sf; cbnr; move: Hcl=> /andP [_ H2].
+    destruct (nth_in_or_default n (snd u) SortFamily.sfType).
+    - eapply forallb_forall in H2; tea.
+    - rewrite e; reflexivity.
+  Qed.
+
+  Lemma subst_instance_sort_closedu s :
+    closedu_universe #|snd u| #|fst u| s -> closedu_universe 0 0 (subst_instance_sort u s).
+  Proof.
+    intros H; destruct s; cbnr.
+    1: move: H=> /andP [? ?]; apply andb_and; split.
+    1,3:now apply subst_instance_sort_family_closedu.
+    now apply subst_instance_universe_levels_closedu.
+  Qed.
+
+  Lemma subst_instance_instance_closedu t :
+    closedu_instance #|snd u| #|fst u| t -> closedu_instance 0 0 (subst_instance_instance u t).
+  Proof.
+    intros [H1 H2]%andP.
+    apply andb_and; split.
+    all: etransitivity; first eapply forallb_map.
+    all: eapply forallb_impl; tea; intros l Hl; cbn.
+    1: apply subst_instance_level_closedu.
+    apply subst_instance_sort_family_closedu.
   Qed.
 End SubstInstanceClosed.
 
 Hint Resolve subst_instance_level_closedu subst_instance_level_expr_closedu
-     subst_instance_univ_closedu subst_instance_instance_closedu : substu.
+     subst_instance_universe_levels_closedu subst_instance_sort_family_closedu
+    subst_instance_sort_closedu subst_instance_instance_closedu : substu.
 
+
+(** ** Printing universes *)
 
 Definition string_of_level (l : Level.t) : string :=
   match l with
@@ -1759,25 +803,79 @@ Definition string_of_level (l : Level.t) : string :=
   end.
 
 Definition string_of_level_expr (e : UnivExpr.t) : string :=
-  let '(l, b) := e in string_of_level l ^ (if b then "+1" else "").
+  let '(l, n) := e in
+  string_of_level l ^ (if n =? 0 then "+" ^ string_of_nat n else "").
 
-Definition string_of_sort (u : Universe.t) :=
+Definition string_of_universe_level (e : UniverseLevel.t) : string :=
+  match UnivExprSet.elements e with
+  | [ e ] => string_of_level_expr e
+  | l => "max(" ^ string_of_list_aux string_of_level_expr ", " l ^ ")"
+  end.
+
+Definition string_of_sort_family (sf : SortFamily.t) :=
+  match sf with
+  | SortFamily.sfType => "Type"
+  | SortFamily.sfGlobal i (* FIXME : should have a name *) => "Sort_" ^ string_of_nat i
+  | SortFamily.sfVar i => "SortVar_" ^ string_of_nat i
+  end.
+
+Definition string_of_sort (u : Sort.t) :=
   match u with
-  | Universe.lSProp => "SProp"
-  | Universe.lProp => "Prop"
-  | Universe.lType l => "Type(" ^ string_of_list string_of_level_expr (UnivExprSet.elements l) ^ ")"
+  | Sort.PredicativeSort sf l =>
+    string_of_sort_family sf ^ "@{" ^ string_of_universe_level l ^ "}"
+  | Sort.ImpredicativeSort sf => string_of_sort_family sf
   end.
 
 Definition string_of_universe_instance u :=
   string_of_list string_of_level u.
 
+Definition string_of_level_list u :=
+  match u with
+  | [] => ""
+  | _ => "@{" ^ print_list string_of_level " " u ^ "}"
+  end.
+
+#[deprecated(note="Use string_of_level_list")]
+Notation print_universe_instance := string_of_level_list.
+
+Definition print_lset t :=
+  print_list string_of_level " " (LevelSet.elements t).
+
+Definition string_of_constraint_type d :=
+  match d with
+  | UnivConstraintType.Le n =>
+    if (n =? 0)%Z then "<=" else
+    if (n =? 1)%Z then "<" else
+    if (n <? 0)%Z then "<=" ^ string_of_nat (Z.to_nat (Z.abs n)) ^ " + "
+    else " + " ^ string_of_nat (Z.to_nat n) ^ " <= "
+  | UnivConstraintType.Eq => "="
+  end.
+
+#[deprecated(note="use string_of_constraint_type")]
+Notation print_constraint_type := string_of_constraint_type.
+
+Definition string_of_constraint '(l1, d, l2) :=
+  string_of_level l1 ^ " " ^ string_of_constraint_type d ^ " " ^ string_of_level l2.
+
+Definition string_of_univ_constraint_set t :=
+  print_list string_of_constraint " /\ " (UnivConstraintSet.elements t).
+
+#[deprecated(note="use string_of_univ_constraint_set")]
+Notation print_constraint_set := string_of_univ_constraint_set.
+
+
+
+
+(** ** Universe Entries *)
+
+(* FIXME : I have no clue what this correspond to *)
 Inductive universes_entry :=
-| Monomorphic_entry (ctx : ContextSet.t)
+| Monomorphic_entry (ctx : UnivContextSet.t)
 | Polymorphic_entry (names : list name) (ctx : UContext.t).
 
 Definition universes_entry_of_decl (u : universes_decl) : universes_entry :=
   match u with
-  | Polymorphic_ctx ctx => Polymorphic_entry (fst ctx) (Universes.AUContext.repr ctx)
+  | Polymorphic_ctx ctx => Polymorphic_entry ctx.1.1 (Universes.AUContext.repr ctx)
   | Monomorphic_ctx ctx => Monomorphic_entry ctx
   end.
 
@@ -1789,159 +887,105 @@ Definition polymorphic_instance uctx :=
 
 
 
-Definition print_universe_instance u :=
-  match u with
-  | [] => ""
-  | _ => "@{" ^ print_list string_of_level " " u ^ "}"
-  end.
 
-Definition print_lset t :=
-  print_list string_of_level " " (LevelSet.elements t).
 
-Definition print_constraint_type d :=
-  match d with
-  | ConstraintType.Le n => 
-    if (n =? 0)%Z then "<=" else 
-    if (n =? 1)%Z then "<" else
-    if (n <? 0)%Z then "<=" ^ string_of_nat (Z.to_nat (Z.abs n)) ^ " + "
-    else " + " ^ string_of_nat (Z.to_nat n) ^ " <= "
-  | ConstraintType.Eq => "="
-  end.
+(** * Properties on the order ? *)
 
-Definition print_constraint_set t :=
-  print_list (fun '(l1, d, l2) => string_of_level l1 ^ " " ^
-                         print_constraint_type d ^ " " ^ string_of_level l2)
-             " /\ " (ConstraintSet.elements t).
- 
-Lemma val_universe_sup_not_prop vv v u :
-  Universe.is_prop v = false -> Universe.is_sprop v = false ->
-  ∑ n, Universe.univ_val vv (Universe.sup u v) = UType n.
-Proof.
-  intros Hp Hsp.
-  destruct u,v;cbn;try discriminate;try lia; try apply val_zero_exprs;
-  eexists; eauto.
-Qed.
+(* Lemma val_universe_sup_not_prop vv v u : *)
+(*   Universe.is_prop v = false -> Universe.is_sprop v = false -> *)
+(*   ∑ n, Universe.univ_val vv (Universe.sup u v) = UType n. *)
+(* Proof. *)
+(*   intros Hp Hsp. *)
+(*   destruct u,v;cbn;try discriminate;try lia; try apply val_zero_exprs; *)
+(*   eexists; eauto. *)
+(* Qed. *)
 
-Lemma univ_le_prop_inv {cf:checker_flags} u : (u <= UProp)%u -> u = UProp.
-Proof. destruct u; simpl; try congruence; auto. Qed.
+(* Lemma univ_le_prop_inv {cf:checker_flags} u : (u <= UProp)%u -> u = UProp. *)
+(* Proof. destruct u; simpl; try congruence; auto. Qed. *)
 
-Lemma univ_le_sprop_inv {cf:checker_flags} u : (u <= USProp)%u -> u = USProp.
-Proof. destruct u; simpl; try congruence; auto. Qed.
+(* Lemma univ_le_sprop_inv {cf:checker_flags} u : (u <= USProp)%u -> u = USProp. *)
+(* Proof. destruct u; simpl; try congruence; auto. Qed. *)
 
-Lemma univ_prop_le_inv {cf:checker_flags} u : (UProp <= u)%u -> 
-  (u = UProp \/ (prop_sub_type /\ exists n, u = UType n)).
-Proof. destruct u; simpl; try congruence; auto.
-  destruct prop_sub_type; firstorder auto.
-  right; split; auto. exists i. auto.
-Qed.
+(* Lemma univ_prop_le_inv {cf:checker_flags} u : (UProp <= u)%u ->  *)
+(*   (u = UProp \/ (prop_sub_type /\ exists n, u = UType n)). *)
+(* Proof. destruct u; simpl; try congruence; auto. *)
+(*   destruct prop_sub_type; firstorder auto. *)
+(*   right; split; auto. exists i. auto. *)
+(* Qed. *)
 
-Ltac cong := intuition congruence.
+(* Ltac cong := intuition congruence. *)
 
-Lemma univ_val_max_mon {cf:checker_flags} u u' v v' : (u <= u')%u -> (UType v <= UType v')%u -> 
-  (univ_val_max u (UType v) <= univ_val_max u' (UType v'))%u.
-Proof.
-  intros.
-  destruct u, u'; simpl in *; auto. lia. lia.
-Qed.
+(* Lemma univ_val_max_mon {cf:checker_flags} u u' v v' : (u <= u')%u -> (UType v <= UType v')%u ->  *)
+(*   (univ_val_max u (UType v) <= univ_val_max u' (UType v'))%u. *)
+(* Proof. *)
+(*   intros. *)
+(*   destruct u, u'; simpl in *; auto. lia. lia. *)
+(* Qed. *)
 
 Lemma leq_universe_product_mon {cf: checker_flags} ϕ u u' v v' :
   leq_universe ϕ u u' ->
   leq_universe ϕ v v' ->
-  leq_universe ϕ (Universe.sort_of_product u v) (Universe.sort_of_product u' v').
+  leq_universe ϕ (UniverseLevel.level_of_product u v) (UniverseLevel.level_of_product u' v').
 Proof.
   unfold leq_universe in *; destruct check_univs; [|trivial].
   intros H1 H2 vv Hv. specialize (H1 _ Hv). specialize (H2 _ Hv).
-  cbn in *. unfold Universe.sort_of_product.
-  destruct (Universe.is_prop v) eqn:e, (Universe.is_prop v') eqn:f;
-    destruct (Universe.is_sprop v) eqn:e1, (Universe.is_sprop v') eqn:f1;
-    rewrite ?val_universe_sup;cbn; rewrite ?val_universe_sup; auto.
-  - destruct v;discriminate.
-  - apply is_prop_val with (v:=vv) in e.
-    specialize (is_prop_and_is_sprop_val_false _ f f1 vv) as [n HH].
-    rewrite e, HH.
-    rewrite e, HH in H2. simpl in H2.
-    simpl. destruct (Universe.univ_val vv u') eqn:eq; simpl; auto.
-  - destruct v';discriminate.
-  - apply is_prop_val with (v:=vv) in f.
-    specialize (is_prop_and_is_sprop_val_false _ e e1 vv) as [n HH].
-    rewrite f in H2. eapply univ_le_prop_inv in H2. cong.
-  - apply is_sprop_val with (v:=vv) in e1.
-    specialize (is_prop_and_is_sprop_val_false _ f f1 vv) as [n HH].
-    rewrite HH, e1 in H2. now simpl in H2.
-  - apply is_sprop_val with (v:=vv) in f1.
-    specialize (is_prop_and_is_sprop_val_false _ e e1 vv) as [n HH].
-    rewrite f1 in H2. apply univ_le_sprop_inv in H2; cong.
-  - specialize (is_prop_and_is_sprop_val_false _ e e1 vv) as [n HH].
-    specialize (is_prop_and_is_sprop_val_false _ f f1 vv) as [n' HH'].
-    rewrite HH, HH'. apply univ_val_max_mon; auto.
-    now rewrite <- HH, <- HH'.
+  cbn in *. unfold UniverseLevel.level_of_product.
+  rewrite 2!val_sup. red in H1, H2 |- *; lia.
 Qed.
 
-Lemma impredicative_product {cf:checker_flags} {ϕ l u} :
-  Universe.is_prop u ->
-  leq_universe ϕ (Universe.sort_of_product l u) u.
-Proof.
-  unfold Universe.sort_of_product.
-  intros ->. reflexivity.
-Qed.
+(* Lemma impredicative_product {cf:checker_flags} {ϕ l u} : *)
+(*   Universe.is_prop u -> *)
+(*   leq_universe ϕ (Universe.sort_of_product l u) u. *)
+(* Proof. *)
+(*   unfold Universe.sort_of_product. *)
+(*   intros ->. reflexivity. *)
+(* Qed. *)
 
-Section UniverseLemmas.
+Section UniverseLevelLemmas.
   Context {cf:checker_flags}.
 
   Ltac unfold_eq_universe
     := unfold eq_universe in *; destruct check_univs; [intros v Hv|trivial].
 
-  Lemma sup0_idem s : Universe.sup0 s s = s.
+  Lemma sup_idem s : UniverseLevel.sup s s = s.
   Proof.
     apply eq_univ'; cbn.
     intro; rewrite !UnivExprSet.union_spec. intuition.
   Qed.
 
-  Lemma sup_idem s : Universe.sup s s = s.
-  Proof.
-    destruct s;cbn;auto.
-    apply f_equal.
-    apply eq_univ'; cbn.
-    intro; rewrite !UnivExprSet.union_spec. intuition.
-  Qed.
+  Lemma level_of_product_idem s
+    : UniverseLevel.level_of_product s s = s.
+  Proof. apply sup_idem. Qed.
 
-  Lemma sort_of_product_idem s
-    : Universe.sort_of_product s s = s.
-  Proof.
-    unfold Universe.sort_of_product.
-    destruct (Universe.is_prop s), (Universe.is_sprop s); trea;cbn.
-    apply sup_idem.
-  Qed.
-
-  Lemma sup0_assoc s1 s2 s3 :
-    Universe.sup0 s1 (Universe.sup0 s2 s3) = Universe.sup0 (Universe.sup0 s1 s2) s3.
+  Lemma sup_assoc s1 s2 s3 :
+    UniverseLevel.sup s1 (UniverseLevel.sup s2 s3) = UniverseLevel.sup (UniverseLevel.sup s1 s2) s3.
   Proof.
     apply eq_univ'; cbn. symmetry; apply UnivExprSetProp.union_assoc.
   Qed.
 
   Instance universe_sup_eq_universe φ :
-    Proper (eq_universe φ ==> eq_universe φ ==> eq_universe φ) Universe.sup.
+    Proper (eq_universe φ ==> eq_universe φ ==> eq_universe φ) UniverseLevel.sup.
   Proof.
     intros s1 s1' H1 s2 s2' H2.
     unfold_eq_universe. specialize (H1 v Hv). specialize (H2 v Hv).
-    rewrite !val_universe_sup.
-    now rewrite H1, H2.
+    rewrite !val_sup.
+    now rewrite -> H1, H2.
   Qed.
 
   Lemma sort_of_product_twice u s :
-    Universe.sort_of_product u (Universe.sort_of_product u s)
-    = Universe.sort_of_product u s.
+    UniverseLevel.level_of_product u (UniverseLevel.level_of_product u s)
+    = UniverseLevel.level_of_product u s.
   Proof.
     destruct u,s;auto.
-    unfold Universe.sort_of_product;cbn.
-    now rewrite sup0_assoc, sup0_idem.
+    unfold UniverseLevel.level_of_product;cbn.
+    now rewrite -> sup_assoc, sup_idem.
   Qed.
-End UniverseLemmas.
+End UniverseLevelLemmas.
 
 
 Section no_prop_leq_type.
   Context {cf:checker_flags}.
-  Context (ϕ : ConstraintSet.t).
+  Context (ϕ : UnivConstraintSet.t).
 
   Lemma succ_inj x y : UnivExpr.succ x = UnivExpr.succ y -> x = y.
   Proof.
@@ -1950,10 +994,10 @@ Section no_prop_leq_type.
   Qed.
 
   Lemma spec_map_succ l x : 
-    UnivExprSet.In x (Universe.map UnivExpr.succ l) <-> 
+    UnivExprSet.In x (UniverseLevel.map UnivExpr.succ l) <-> 
     exists x', UnivExprSet.In x' l /\ x = UnivExpr.succ x'.
   Proof.
-    rewrite Universe.map_spec. reflexivity.
+    rewrite UniverseLevel.map_spec. reflexivity.
   Qed.
 
   Lemma val_succ v l : val v (UnivExpr.succ l) = val v l + 1.
@@ -1961,9 +1005,9 @@ Section no_prop_leq_type.
     destruct l as []; simpl. cbn. lia. 
   Qed.
 
-  Lemma val_map_succ v l : val v (Universe.map UnivExpr.succ l) = val v l + 1.
+  Lemma val_map_succ v l : val v (UniverseLevel.map UnivExpr.succ l) = val v l + 1.
   Proof.
-    remember (Universe.map UnivExpr.succ l) eqn:eq.
+    remember (UniverseLevel.map UnivExpr.succ l) eqn:eq.
     pose proof (spec_map_succ l). rewrite <- eq in H.
     clear eq.
     destruct (val_In_max l v) as [max [inmax eqv]]. rewrite <-eqv.
@@ -1976,136 +1020,135 @@ Section no_prop_leq_type.
     exists max; split; auto.
     now rewrite val_succ.
   Qed.
-  
+
   Lemma leq_universe_super u u' :
     leq_universe ϕ u u' ->
-    leq_universe ϕ (Universe.super u) (Universe.super u').
+    leq_universe ϕ (UniverseLevel.super u) (UniverseLevel.super u').
   Proof.
     unfold leq_universe. destruct check_univs; [|trivial].
     intros H v Hv. specialize (H v Hv). simpl in *.
-    destruct u as [| |], u' as  [| |]; lled; cbn -[Z.add] in *; try lia;
-    rewrite !val_map_succ; lia.
+    rewrite !val_map_succ; red in H |- *; lia.
   Qed.
 
-  Lemma leq_universe_props u1 u2 :
-    check_univs ->
-    consistent ϕ ->
-    leq_universe ϕ u1 u2 ->
-    match u1, u2 with
-    | Universe.lProp, Universe.lProp => True
-    | Universe.lSProp, Universe.lSProp => True
-    | Universe.lProp, Universe.lSProp => False
-    | Universe.lSProp, Universe.lProp => False
-    | Universe.lProp, Universe.lType _ => prop_sub_type
-    | Universe.lSProp, Universe.lType _ => False
-    | Universe.lType l, Universe.lType l' => True
-    | Universe.lType _, _ => False
-    end.
-  Proof.
-    intros cu [v Hv].
-    unfold leq_universe. rewrite cu.
-    intros Hle. specialize (Hle _ Hv).
-    destruct u1, u2; simpl; auto.
-    simpl in Hle. now destruct prop_sub_type.
-  Qed.
+  (* Lemma leq_universe_props u1 u2 : *)
+  (*   check_univs -> *)
+  (*   consistent ϕ -> *)
+  (*   leq_universe ϕ u1 u2 -> *)
+  (*   match u1, u2 with *)
+  (*   | UniverseLevel.lProp, UniverseLevel.lProp => True *)
+  (*   | UniverseLevel.lSProp, UniverseLevel.lSProp => True *)
+  (*   | UniverseLevel.lProp, UniverseLevel.lSProp => False *)
+  (*   | UniverseLevel.lSProp, UniverseLevel.lProp => False *)
+  (*   | UniverseLevel.lProp, UniverseLevel.lType _ => prop_sub_type *)
+  (*   | UniverseLevel.lSProp, UniverseLevel.lType _ => False *)
+  (*   | UniverseLevel.lType l, UniverseLevel.lType l' => True *)
+  (*   | UniverseLevel.lType _, _ => False *)
+  (*   end. *)
+  (* Proof. *)
+  (*   intros cu [v Hv]. *)
+  (*   unfold leq_universe. rewrite cu. *)
+  (*   intros Hle. specialize (Hle _ Hv). *)
+  (*   destruct u1, u2; simpl; auto. *)
+  (*   simpl in Hle. now destruct prop_sub_type. *)
+  (* Qed. *)
 
-  Lemma leq_universe_prop_r u1 u2 :
-    check_univs ->
-    consistent ϕ ->
-    leq_universe ϕ u1 u2 ->
-    Universe.is_prop u2 -> Universe.is_prop u1.
-  Proof.
-    intros Hcf cu le.
-    apply leq_universe_props in le; auto.
-    destruct u1, u2; simpl in *; auto.
-  Qed.
+  (* Lemma leq_universe_prop_r u1 u2 : *)
+  (*   check_univs -> *)
+  (*   consistent ϕ -> *)
+  (*   leq_universe ϕ u1 u2 -> *)
+  (*   UniverseLevel.is_prop u2 -> UniverseLevel.is_prop u1. *)
+  (* Proof. *)
+  (*   intros Hcf cu le. *)
+  (*   apply leq_universe_props in le; auto. *)
+  (*   destruct u1, u2; simpl in *; auto. *)
+  (* Qed. *)
 
-  Lemma leq_universe_sprop_r u1 u2 :
-    check_univs ->
-    consistent ϕ ->
-    leq_universe ϕ u1 u2 ->
-    Universe.is_sprop u2 -> Universe.is_sprop u1.
-  Proof.
-    intros Hcf cu le.
-    apply leq_universe_props in le; auto.
-    destruct u1, u2; simpl in *; auto.
-  Qed.
+  (* Lemma leq_universe_sprop_r u1 u2 : *)
+  (*   check_univs -> *)
+  (*   consistent ϕ -> *)
+  (*   leq_universe ϕ u1 u2 -> *)
+  (*   UniverseLevel.is_sprop u2 -> UniverseLevel.is_sprop u1. *)
+  (* Proof. *)
+  (*   intros Hcf cu le. *)
+  (*   apply leq_universe_props in le; auto. *)
+  (*   destruct u1, u2; simpl in *; auto. *)
+  (* Qed. *)
   
-  Lemma leq_universe_prop_no_prop_sub_type u1 u2 :
-    check_univs ->
-    prop_sub_type = false ->
-    consistent ϕ ->
-    leq_universe ϕ u1 u2 ->
-    Universe.is_prop u1 -> Universe.is_prop u2.
-  Proof.
-    intros Hcf cu ps le.
-    apply leq_universe_props in le; auto.
-    destruct u1, u2; simpl in *; auto.
-    cong.
-  Qed.
+  (* Lemma leq_universe_prop_no_prop_sub_type u1 u2 : *)
+  (*   check_univs -> *)
+  (*   prop_sub_type = false -> *)
+  (*   consistent ϕ -> *)
+  (*   leq_universe ϕ u1 u2 -> *)
+  (*   UniverseLevel.is_prop u1 -> UniverseLevel.is_prop u2. *)
+  (* Proof. *)
+  (*   intros Hcf cu ps le. *)
+  (*   apply leq_universe_props in le; auto. *)
+  (*   destruct u1, u2; simpl in *; auto. *)
+  (*   cong. *)
+  (* Qed. *)
 
-  Lemma leq_universe_sprop_l u1 u2 :
-    check_univs ->
-    consistent ϕ ->
-    leq_universe ϕ u1 u2 ->
-    Universe.is_sprop u1 -> Universe.is_sprop u2.
-  Proof.
-    intros Hcf cu le.
-    apply leq_universe_props in le; auto.
-    destruct u1, u2; simpl in *; auto.
-  Qed.
+  (* Lemma leq_universe_sprop_l u1 u2 : *)
+  (*   check_univs -> *)
+  (*   consistent ϕ -> *)
+  (*   leq_universe ϕ u1 u2 -> *)
+  (*   UniverseLevel.is_sprop u1 -> UniverseLevel.is_sprop u2. *)
+  (* Proof. *)
+  (*   intros Hcf cu le. *)
+  (*   apply leq_universe_props in le; auto. *)
+  (*   destruct u1, u2; simpl in *; auto. *)
+  (* Qed. *)
 
-  Hint Resolve leq_universe_sprop_l leq_universe_sprop_r
-       leq_universe_prop_r
-       leq_universe_prop_no_prop_sub_type
-       : univ_lemmas.
+  (* Hint Resolve leq_universe_sprop_l leq_universe_sprop_r *)
+  (*      leq_universe_prop_r *)
+  (*      leq_universe_prop_no_prop_sub_type *)
+  (*      : univ_lemmas. *)
   
-  Lemma leq_prop_prop {l l'} :
-    Universe.is_prop l -> Universe.is_prop l' ->
-    leq_universe ϕ l l'.
-  Proof.
-    red. destruct check_univs; [|trivial].
-    intros H1 H2 v Hv. eapply is_prop_val in H1; eapply is_prop_val in H2.
-    rewrite H1, H2. lled; lia.
-  Qed.
+  (* Lemma leq_prop_prop {l l'} : *)
+  (*   UniverseLevel.is_prop l -> UniverseLevel.is_prop l' -> *)
+  (*   leq_universe ϕ l l'. *)
+  (* Proof. *)
+  (*   red. destruct check_univs; [|trivial]. *)
+  (*   intros H1 H2 v Hv. eapply is_prop_val in H1; eapply is_prop_val in H2. *)
+  (*   rewrite H1, H2. lle; lia. *)
+  (* Qed. *)
 
-  Lemma leq_sprop_sprop {l l'} :
-    Universe.is_sprop l -> Universe.is_sprop l' ->
-    leq_universe ϕ l l'.
-  Proof.
-    red. destruct check_univs; [|trivial].
-    intros H1 H2 v Hv. eapply is_sprop_val in H1; eapply is_sprop_val in H2.
-    rewrite H1, H2. lled; lia.
-  Qed.
+  (* Lemma leq_sprop_sprop {l l'} : *)
+  (*   UniverseLevel.is_sprop l -> UniverseLevel.is_sprop l' -> *)
+  (*   leq_universe ϕ l l'. *)
+  (* Proof. *)
+  (*   red. destruct check_univs; [|trivial]. *)
+  (*   intros H1 H2 v Hv. eapply is_sprop_val in H1; eapply is_sprop_val in H2. *)
+  (*   rewrite H1, H2. lle; lia. *)
+  (* Qed. *)
   
-  Lemma leq_prop_is_prop_sprop {x s} :
-    check_univs ->
-    prop_sub_type = false ->
-    consistent ϕ ->
-    leq_universe ϕ x s ->
-    (Universe.is_prop s \/ Universe.is_sprop s <-> Universe.is_prop x \/ Universe.is_sprop x).
-  Proof.
-    intros H H0 H1 H2; split;intros Hor; destruct Hor; eauto with univ_lemmas.
-  Qed.
+  (* Lemma leq_prop_is_prop_sprop {x s} : *)
+  (*   check_univs -> *)
+  (*   prop_sub_type = false -> *)
+  (*   consistent ϕ -> *)
+  (*   leq_universe ϕ x s -> *)
+  (*   (UniverseLevel.is_prop s \/ UniverseLevel.is_sprop s <-> UniverseLevel.is_prop x \/ UniverseLevel.is_sprop x). *)
+  (* Proof. *)
+  (*   intros H H0 H1 H2; split;intros Hor; destruct Hor; eauto with univ_lemmas. *)
+  (* Qed. *)
 
-  Lemma is_prop_gt l l' :
-    check_univs ->
-    consistent ϕ ->
-    leq_universe ϕ (Universe.super l) l' -> Universe.is_prop l' -> False.
-  Proof.
-    intros Hcf [v Hv] H1 H2. unfold leq_universe in *; rewrite Hcf in *.
-    eapply is_prop_val with (v:=v) in H2. specialize (H1 _ Hv).
-    rewrite H2 in H1. destruct l as [| |]; destruct l'; lled; cbn -[Z.add] in *; lia.
-  Qed.
+  (* Lemma is_prop_gt l l' : *)
+  (*   check_univs -> *)
+  (*   consistent ϕ -> *)
+  (*   leq_universe ϕ (UniverseLevel.super l) l' -> UniverseLevel.is_prop l' -> False. *)
+  (* Proof. *)
+  (*   intros Hcf [v Hv] H1 H2. unfold leq_universe in *; rewrite Hcf in *. *)
+  (*   eapply is_prop_val with (v:=v) in H2. specialize (H1 _ Hv). *)
+  (*   rewrite H2 in H1. destruct l as [| |]; destruct l'; lle; cbn -[Z.add] in *; lia. *)
+  (* Qed. *)
   
-  Lemma is_sprop_gt l l' :
-    check_univs ->
-    consistent ϕ ->
-    leq_universe ϕ (Universe.super l) l' -> Universe.is_sprop l' -> False.
-  Proof.
-    intros Hcf [v Hv] H1 H2. unfold leq_universe in *; rewrite Hcf in *.
-    eapply is_sprop_val with (v:=v) in H2. specialize (H1 _ Hv).
-    rewrite H2 in H1. destruct l as [| |]; destruct l'; lled; cbn -[Z.add] in *; lia.
-  Qed.
+  (* Lemma is_sprop_gt l l' : *)
+  (*   check_univs -> *)
+  (*   consistent ϕ -> *)
+  (*   leq_universe ϕ (UniverseLevel.super l) l' -> UniverseLevel.is_sprop l' -> False. *)
+  (* Proof. *)
+  (*   intros Hcf [v Hv] H1 H2. unfold leq_universe in *; rewrite Hcf in *. *)
+  (*   eapply is_sprop_val with (v:=v) in H2. specialize (H1 _ Hv). *)
+  (*   rewrite H2 in H1. destruct l as [| |]; destruct l'; lle; cbn -[Z.add] in *; lia. *)
+  (* Qed. *)
 
 End no_prop_leq_type.
