template-coq/theories/Levels.v
@@ -1,0 +1,955 @@
+From Coq Require Import MSetList MSetFacts MSetProperties MSetDecide.
+From MetaCoq.Template Require Import utils BasicAst config.
+
+Local Open Scope nat_scope.
+Local Open Scope string_scope2.
+
+
+Ltac absurd :=
+  match goal with
+  | [H : False |- _] => elim H
+  end.
+Hint Extern 10 => absurd : core.
+
+(** * Valuations *)
+
+(** A valuation is a universe level (nat) given for each
+    universe variable (Level.t).
+    It is >= for polymorphic universes and > 0 for monomorphic universes. *)
+Record valuation :=
+  { valuation_mono : string -> positive ;
+    valuation_poly : nat -> nat }.
+
+Class Evaluable (A : Type) := val : valuation -> A -> nat.
+
+(** Levels are Set or Level or Var *)
+Module Level.
+  Inductive t_ : Set :=
+  | lSet
+  | Level (_ : string)
+  | Var (_ : nat) (* these are debruijn indices in the local universe polymorphic context *).
+
+  Definition t := t_.
+
+  Definition is_small (x : t) :=
+    match x with
+    | lSet => true
+    | _ => false
+    end.
+
+  Definition is_set (x : t) :=
+    match x with
+    | lSet => true
+    | _ => false
+    end.
+
+  Definition is_var (l : t) :=
+    match l with
+    | Var _ => true
+    | _ => false
+    end.
+
+  Global Instance Evaluable : Evaluable t
+    := fun v l => match l with
+               | lSet =>  (0%nat)
+               | Level s => (Pos.to_nat (v.(valuation_mono) s))
+               | Var x => (v.(valuation_poly) x)
+               end.
+
+
+  Definition compare (l1 l2 : t) : comparison :=
+    match l1, l2 with
+    | lSet, lSet => Eq
+    | lSet, _ => Lt
+    | _, lSet => Gt
+    | Level s1, Level s2 => string_compare s1 s2
+    | Level _, _ => Lt
+    | _, Level _ => Gt
+    | Var n, Var m => Nat.compare n m
+    end.
+
+  Definition eq : t -> t -> Prop := eq.
+  Definition eq_equiv : Equivalence eq := _.
+
+  Definition eq_dec (l1 l2 : t) : {l1 = l2}+{l1 <> l2}.
+  Proof.
+    decide equality. apply string_dec. apply Peano_dec.eq_nat_dec.
+  Defined.
+
+  Inductive lt_ : t -> t -> Prop :=
+  | ltSetLevel s : lt_ lSet (Level s)
+  | ltSetVar n : lt_ lSet (Var n)
+  | ltLevelLevel s s' : string_lt s s' -> lt_ (Level s) (Level s')
+  | ltLevelVar s n : lt_ (Level s) (Var n)
+  | ltVarVar n n' : Nat.lt n n' -> lt_ (Var n) (Var n').
+
+  Definition lt := lt_.
+
+  Definition lt_strorder : StrictOrder lt.
+  Proof.
+    constructor.
+    - intros [| |] X; inversion X.
+      eapply string_lt_irreflexive; tea.
+      eapply Nat.lt_irrefl; tea.
+    - intros [| |] [| |] [| |] X1 X2;
+        inversion X1; inversion X2; constructor.
+      eapply transitive_string_lt; tea.
+      etransitivity; tea.
+  Qed.
+
+  Definition lt_compat : Proper (eq ==> eq ==> iff) lt.
+  Proof.
+    intros x y e z t e'. unfold eq in *; subst. reflexivity.
+  Qed.
+
+  Definition compare_spec :
+    forall x y : t, CompareSpec (x = y) (lt x y) (lt y x) (compare x y).
+  Proof.
+    intros [] []; repeat constructor.
+    - eapply CompareSpec_Proper.
+      5: eapply CompareSpec_string. 4: reflexivity.
+      all: split; [now inversion 1|]. now intros ->.
+      all: intro; now constructor.
+    - eapply CompareSpec_Proper.
+      5: eapply Nat.compare_spec. 4: reflexivity.
+      all: split; [now inversion 1|]. now intros ->.
+      all: intro; now constructor.
+  Qed.
+
+  (* Bonus *)
+  Definition eqb (l1 l2 : Level.t) : bool
+    := match compare l1 l2 with Eq => true | _ => false end.
+
+  Global Instance eqb_refl : Reflexive eqb.
+  Proof.
+    intros []; unfold eqb; cbnr.
+    - rewrite (ssreflect.iffRL (string_compare_eq s s)). all: auto.
+    - rewrite Nat.compare_refl. reflexivity.
+  Qed.
+
+  Lemma eqb_spec l l' : reflect (eq l l') (eqb l l').
+  Proof.
+    destruct l, l'; cbn; try constructor; try reflexivity; try discriminate.
+    - apply iff_reflect. unfold eqb; cbn.
+      destruct (CompareSpec_string s s0); split; intro HH;
+        try reflexivity; try discriminate; try congruence.
+      all: inversion HH; subst; now apply string_lt_irreflexive in H.
+    - apply iff_reflect. unfold eqb; cbn.
+      destruct (Nat.compare_spec n n0); split; intro HH;
+        try reflexivity; try discriminate; try congruence.
+      all: inversion HH; subst; now apply Nat.lt_irrefl in H.
+  Qed.
+
+  Definition eq_leibniz (x y : t) : eq x y -> x = y := id.
+
+End Level.
+
+Module LevelSet := MSetList.MakeWithLeibniz Level.
+Module LevelSetFact := WFactsOn Level LevelSet.
+Module LevelSetProp := WPropertiesOn Level LevelSet.
+Module LevelSetDecide := WDecide (LevelSet).
+Ltac lsets := LevelSetDecide.fsetdec.
+
+Definition LevelSet_pair x y
+  := LevelSet.add y (LevelSet.singleton x).
+
+Lemma LevelSet_pair_In x y z :
+  LevelSet.In x (LevelSet_pair y z) -> x = y \/ x = z.
+Proof.
+  intro H. apply LevelSetFact.add_iff in H.
+  destruct H; [intuition|].
+  apply LevelSetFact.singleton_1 in H; intuition.
+Qed.
+
+Definition LevelSet_mem_union (s s' : LevelSet.t) x :
+  LevelSet.mem x (LevelSet.union s s') <-> LevelSet.mem x s \/ LevelSet.mem x s'.
+Proof.
+  rewrite LevelSetFact.union_b.
+  apply orb_true_iff.
+Qed.
+
+
+Module UnivExpr.
+  (* npe = no prop expression *)
+  (* (u,k) represents u + k *)
+  Definition t := (Level.t * nat)%type.
+
+  Global Instance Evaluable : Evaluable t
+    := fun v l => (snd l + val v (fst l)).
+
+  Definition succ (l : t) := (fst l, S (snd l)).
+
+  Definition get_level (e : t) : Level.t := fst e.
+
+  Definition get_noprop_deprecated (e : UnivExpr.t) := Some (fst e).
+  #[deprecated(note="Is that used ?")]
+  Notation get_noprop := get_noprop_deprecated.
+
+  Definition is_small (e : t) : bool :=
+    match e with
+    | (Level.lSet, 0%nat) => true
+    | _  => false
+    end.
+
+  Definition is_level (e : t) : bool :=
+    match e with
+    | (_, 0%nat) => true
+    | _  => false
+    end.
+
+  Definition make (l : Level.t) : t := (l, 0%nat).
+
+  Definition set : t := (Level.lSet, 0%nat).
+  Definition type1 : t := (Level.lSet, 1%nat).
+
+  (* Used for (un)quoting. *)
+  Definition from_kernel_repr (e : Level.t * bool) : t
+    := (e.1, if e.2 then 1%nat else 0%nat).
+
+  Definition to_kernel_repr (e : t) : Level.t * bool
+    := match e with
+       | (l, b) => (l, match b with 0%nat => false | _ => true end)
+       end.
+
+  Definition eq : t -> t -> Prop := eq.
+
+  Definition eq_equiv : Equivalence eq := _.
+
+  Inductive lt_ : t -> t -> Prop :=
+  | ltUnivExpr1 l n n' : (n < n')%nat -> lt_ (l, n) (l, n')
+  | ltUnivExpr2 l l' b b' : Level.lt l l' -> lt_ (l, b) (l', b').
+
+  Definition lt := lt_.
+
+  Global Instance lt_strorder : StrictOrder lt.
+  Proof.
+    constructor.
+    - intros x X; inversion X. subst. lia. subst.
+      eapply Level.lt_strorder; eassumption.
+    - intros x y z X1 X2; invs X1; invs X2; constructor; tea.
+      etransitivity; tea.
+      etransitivity; tea.
+  Qed.
+
+  Definition lt_compat : Proper (Logic.eq ==> Logic.eq ==> iff) lt.
+    intros x x' H1 y y' H2; now rewrite H1, H2.
+  Qed.
+
+  Definition compare (x y : t) : comparison :=
+    match x, y with
+    | (l1, b1), (l2, b2) =>
+      match Level.compare l1 l2 with
+      | Eq => Nat.compare b1 b2
+      | x => x
+      end
+    end.
+
+  Definition compare_spec :
+    forall x y : t, CompareSpec (x = y) (lt x y) (lt y x) (compare x y).
+  Proof.
+    intros [? ?] [? ?]; cbn; repeat constructor.
+    destruct (Level.compare_spec t0 t1); repeat constructor; tas.
+    subst.
+    destruct (Nat.compare_spec n n0); repeat constructor; tas. congruence.
+  Qed.
+
+  Definition eq_dec (l1 l2 : t) : {l1 = l2} + {l1 <> l2}.
+  Proof.
+    repeat decide equality.
+  Defined.
+
+  Definition eq_leibniz (x y : t) : eq x y -> x = y := id.
+
+  Lemma val_make v l
+    : val v (UnivExpr.make l) = val v l.
+  Proof.
+    destruct l eqn:H; cbnr.
+  Qed.
+
+  Lemma val_make_npl v (l : Level.t)
+    : val v (UnivExpr.make l) = val v l.
+  Proof.
+    destruct l; cbnr.
+  Qed.
+
+End UnivExpr.
+
+Module UnivExprSet := MSetList.MakeWithLeibniz UnivExpr.
+Module UnivExprSetFact := WFactsOn UnivExpr UnivExprSet.
+Module UnivExprSetProp := WPropertiesOn UnivExpr UnivExprSet.
+
+Module UniverseLevel.
+  (** A universe level is a list of universe expressions which is:
+        - sorted
+        - without duplicate
+        - non empty
+   It represents the max of its constituents. *)
+  Record t_ := { t_set : UnivExprSet.t ;
+                 t_ne  : UnivExprSet.is_empty t_set = false }.
+
+
+  Definition t := t_.
+
+  Coercion t_set : t_ >-> UnivExprSet.t.
+
+  Definition eq : t -> t -> Prop := eq.
+  Definition eq_equiv : Equivalence eq := _.
+
+
+  Definition lt (x y : t) := UnivExprSet.lt x y.
+
+  Lemma lt_strorder : StrictOrder lt.
+  Proof.
+    constructor.
+    - intros [] ?; now eapply irreflexivity.
+    - intros [] [] [] ? ?; unfold lt in *. now etransitivity.
+  Qed.
+
+  Lemma lt_compat : Proper (eq ==> eq ==> iff) lt.
+  Proof. red; intros; subst; reflexivity. Qed.
+
+
+  Definition compare (e1 e2 : t) : comparison :=
+    UnivExprSet.compare e1 e2.
+
+  Definition eq_dec (e1 e2 : t) : {e1 = e2} +  {e1 <> e2}.
+  Proof.
+    destruct (UnivExprSet.eq_dec e1 e2) as [eq%UnivExprSet.eq_leibniz|neq].
+    2: right; intros ?; now apply neq.
+    left; destruct e1 as [e1 ne1]; destruct e2 as [e2 ne2]; cbn in *.
+    revert ne1 ne2; rewrite eq; intros; f_equal; apply uip_bool.
+  Qed.
+
+  Lemma compare_spec :
+    forall x y : t, CompareSpec (x = y) (lt x y) (lt y x) (compare x y).
+  Proof.
+    intros [] [].
+    eapply CompareSpec_Proper.
+    5: eapply UnivExprSet.compare_spec.
+    4: reflexivity. 2,3: reflexivity.
+    split. 1:now intros [= ->].
+    cbn; intros ->%UnivExprSet.eq_leibniz; f_equal; apply uip_bool.
+  Qed.
+
+  Definition eq_leibniz (x y : t) : eq x y -> x = y := id.
+
+  Definition eqb (e1 e2 : t) : bool :=
+    UnivExprSet.equal e1.(t_set) e2.(t_set).
+
+  Definition make' (e : UnivExpr.t) : t
+    := {| t_set := UnivExprSet.singleton e;
+          t_ne := eq_refl |}.
+
+  (** Create a universe representing the given level. *)
+  Definition make (l : Level.t) : t :=
+    make' (UnivExpr.make l).
+
+  Definition of_expr e := make' e.
+
+  Lemma not_Empty_is_empty s :
+    ~ UnivExprSet.Empty s -> UnivExprSet.is_empty s = false.
+  Proof.
+    intro H. apply not_true_is_false. intro H'.
+    apply H. now apply UnivExprSetFact.is_empty_2 in H'.
+  Qed.
+
+  Program Definition add (e : UnivExpr.t) (u : t) : t
+    := {| t_set := UnivExprSet.add e u |}.
+  Next Obligation.
+    apply not_Empty_is_empty; intro H.
+    eapply H. eapply UnivExprSet.add_spec.
+    left; reflexivity.
+  Qed.
+
+  #[deprecated(note="use add instead")]
+  Notation add_to_exprs := add.
+
+  Lemma add_spec e u e' :
+    UnivExprSet.In e' (add e u) <-> e' = e \/ UnivExprSet.In e' u.
+  Proof.
+    apply UnivExprSet.add_spec.
+  Qed.
+
+  Definition add_list : list UnivExpr.t -> t -> t
+    := List.fold_left (fun u e => add e u).
+
+  Lemma add_list_spec l u e :
+    UnivExprSet.In e (add_list l u) <-> In e l \/ UnivExprSet.In e u.
+  Proof.
+    unfold add_list. rewrite <- fold_left_rev_right.
+    etransitivity. 2:{ eapply or_iff_compat_r. etransitivity.
+                       2: apply @InA_In_eq with (A:=UnivExpr.t).
+                       eapply InA_rev. }
+    induction (List.rev l); cbn.
+    - split. intuition. intros [H|H]; tas. invs H.
+    - split.
+      + intro H. apply add_spec in H. destruct H as [H|H].
+        * left. now constructor.
+        * apply IHl0 in H. destruct H as [H|H]; [left|now right].
+          now constructor 2.
+      + intros [H|H]. inv H.
+        * apply add_spec; now left.
+        * apply add_spec; right. apply IHl0. now left.
+        * apply add_spec; right. apply IHl0. now right.
+  Qed.
+
+  #[deprecated(note="Use add_list instead")]
+  Notation add_list_to_exprs := add_list.
+
+  (** Test if the universe is a lub of levels or contains +n's. *)
+  Definition is_levels (u : t) : bool :=
+      UnivExprSet.for_all UnivExpr.is_level u.
+
+  (** Test if the universe is a level or an algebraic universe. *)
+  Definition is_level (u : t) : bool :=
+    (UnivExprSet.cardinal u =? 1)%nat && is_levels u.
+
+  Definition is_small (u : t) : bool :=
+    UnivExprSet.for_all UnivExpr.is_small u .
+
+  #[deprecated(note="Should only be used for predicative sorts")]
+  Notation is_sprop := (fun (u : t) => false).
+
+  #[deprecated(note="Should only be used for predicative sorts")]
+  Notation is_prop := (fun (u : t) => false).
+
+  Definition type0 : t := make Level.lSet.
+  Definition type1 : t := make' UnivExpr.type1.
+
+  (* Used for quoting. *)
+  Definition from_kernel_repr (e : Level.t * bool) (es : list (Level.t * bool)) : t
+    := add_list (map UnivExpr.from_kernel_repr es)
+                (make' (UnivExpr.from_kernel_repr e)).
+
+
+  (** The non empty / sorted / without dup list of univ expressions, the
+      components of the pair are the head and the tail of the (non empty) list *)
+  Program Definition exprs (u : t) : UnivExpr.t * list UnivExpr.t
+    := match UnivExprSet.elements u with
+       | [] => False_rect _ _
+       | e :: l => (e, l)
+       end.
+  Next Obligation.
+    destruct u as [u1 u2]; cbn in *. revert u2.
+    apply eq_true_false_abs.
+    unfold UnivExprSet.is_empty, UnivExprSet.Raw.is_empty,
+    UnivExprSet.elements, UnivExprSet.Raw.elements in *.
+    rewrite <- Heq_anonymous; reflexivity.
+  Qed.
+
+  Lemma exprs_make' e : exprs (make' e) = (e, []).
+  Proof. reflexivity. Defined.
+
+  (* Lemma exprs_make l : Universe.exprs (Universe.make l) = (UnivExpr.make l, []). *)
+  (* Proof. reflexivity. Defined. *)
+
+
+  Lemma exprs_spec u :
+    let '(e, u') := exprs u in
+    e :: u' = UnivExprSet.elements u.
+  Proof.
+    destruct u as [u1 u2].
+    pose (l := UnivExprSet.elements u1).
+    change (let '(e, u') :=
+                match l return l = UnivExprSet.elements u1 -> _ with
+                | [] => fun Heq_anonymous : [] = _ u1 =>
+                    False_rect (UnivExpr.t × list UnivExpr.t)
+                               (exprs_obligation_1
+                                  {| t_set := u1; t_ne := u2 |}
+                                  Heq_anonymous)
+                | e :: l0 => fun _ : e :: l0 = _ u1 => (e, l0)
+                end eq_refl in e :: u' = UnivExprSet.elements  u1).
+    set (e := eq_refl). clearbody e. change (l = UnivExprSet.elements u1) in e.
+    destruct l.
+    - exfalso. revert u2. apply eq_true_false_abs.
+      unfold UnivExprSet.is_empty, UnivExprSet.Raw.is_empty,
+      UnivExprSet.elements, UnivExprSet.Raw.elements in *.
+      rewrite <- e; reflexivity.
+    - assumption.
+  Qed.
+
+  Lemma exprs_spec' u :
+    (exprs u).1 :: (exprs u).2 = UnivExprSet.elements u.
+  Proof.
+    pose proof (exprs_spec u).
+    now destruct (exprs u).
+  Qed.
+
+  Lemma In_exprs (u : t) (e : UnivExpr.t) :
+    UnivExprSet.In e u
+    <-> e = (exprs u).1 \/ In e (exprs u).2.
+  Proof.
+    etransitivity. symmetry. apply UnivExprSet.elements_spec1.
+    pose proof (exprs_spec' u) as H.
+    destruct (exprs u) as [e' l]; cbn in *.
+    rewrite <- H; clear. etransitivity. apply InA_cons.
+    eapply or_iff_compat_l. apply InA_In_eq.
+  Qed.
+
+  Lemma In_exprs_rev (u : t) (e : UnivExpr.t) :
+    UnivExprSet.In e u
+    <-> e = (exprs u).1 \/ In e (List.rev (exprs u).2).
+  Proof.
+    etransitivity. eapply In_exprs.
+    apply or_iff_compat_l. apply in_rev.
+  Qed.
+
+  Definition map (f : UnivExpr.t -> UnivExpr.t) (u : t) : t :=
+    let '(e, l) := exprs u in
+    add_list (List.map f l) (make' (f e)).
+
+  Lemma map_spec f u e :
+    UnivExprSet.In e (map f u) <-> exists e0, UnivExprSet.In e0 u /\ e = (f e0).
+  Proof.
+    unfold map. symmetry. etransitivity.
+    { eapply iff_ex; intro. eapply and_iff_compat_r. eapply In_exprs. }
+    destruct (exprs u) as [e' l]; cbn in *.
+    symmetry. etransitivity. eapply add_list_spec.
+    etransitivity. eapply or_iff_compat_l. apply UnivExprSet.singleton_spec.
+    etransitivity. eapply or_iff_compat_r.
+    apply in_map_iff. clear u. split.
+    - intros [[e0 []]|H].
+      + exists e0. split. right; tas. congruence.
+      + exists e'. split; tas. left; reflexivity.
+    - intros [xx [[H|H] ?]].
+      + right. congruence.
+      + left. exists xx. split; tas; congruence.
+  Qed.
+
+  (** The universe strictly above FOR TYPING (not cumulativity) *)
+
+  Definition super (l : t) : t :=
+    map UnivExpr.succ l.
+
+  (** The l.u.b. of 2 non-prop universe sets *)
+  Program Definition sup (u v : t) : t :=
+    {| t_set := UnivExprSet.union u v |}.
+  Next Obligation.
+    apply not_Empty_is_empty; intro H.
+    assert (HH: UnivExprSet.Empty u). {
+      intros x Hx. apply (H x).
+      eapply UnivExprSet.union_spec. now left. }
+    apply UnivExprSetFact.is_empty_1 in HH.
+    rewrite t_ne in HH; discriminate.
+  Qed.
+
+
+  Definition get_univ_exprs (u : t) (H1 : is_prop u = false) (H2 : is_sprop u = false) : t.
+  Proof. easy. Defined.
+
+  (** Type of a product *)
+  Definition level_of_product (domsort rangsort : t) :=
+    sup domsort rangsort.
+
+  Lemma eqb_refl u : eqb u u.
+  Proof.
+    destruct u;auto.
+    now apply UnivExprSet.equal_spec.
+  Qed.
+
+  Lemma elements_not_empty (u : t) : UnivExprSet.elements u <> [].
+  Proof.
+    destruct u as [u1 u2]; cbn; intro e.
+    unfold UnivExprSet.is_empty, UnivExprSet.elements,
+    UnivExprSet.Raw.elements in *.
+    rewrite e in u2; discriminate.
+  Qed.
+
+  Definition get_is_level (u : t) : option Level.t :=
+    match UnivExprSet.elements u with
+      [(l, 0%nat)] => Some l
+    | _ => None
+    end.
+
+  Global Instance Evaluable' : Evaluable t
+    := fun v u => let '(e, u) := exprs u in
+               List.fold_left (fun n e => Nat.max (val v e) n) u (val v e).
+
+  Lemma val_make' v e
+    : val v (make' e) = val v e.
+  Proof.
+    reflexivity.
+  Qed.
+
+  Lemma make_inj x y :
+    make x = make y -> x = y.
+  Proof.
+    destruct x, y; try now inversion 1.
+  Qed.
+
+End UniverseLevel.
+
+#[deprecated(note="No more propositional levels")]
+Notation is_propositional u := (fun u => false).
+
+(** This coercion allows to see the universes as a [UnivExprSet.t] *)
+Coercion UniverseLevel.t_set : UniverseLevel.t_ >-> UnivExprSet.t.
+
+Declare Scope univ_scope.
+Delimit Scope univ_scope with u.
+
+
+(** ** Properties of valuation on universe levels *)
+
+Ltac u :=
+ change LevelSet.elt with Level.t in *;
+ change UnivExprSet.elt with UnivExpr.t in *.
+
+Lemma val_fold_right (u : UniverseLevel.t) v :
+  val v u = fold_right (fun e x => Nat.max (val v e) x) (val v (UniverseLevel.exprs u).1)
+                       (List.rev (UniverseLevel.exprs u).2).
+Proof.
+  unfold val at 1, UniverseLevel.Evaluable'.
+  destruct (UniverseLevel.exprs u).
+  now rewrite fold_left_rev_right.
+Qed.
+
+Lemma val_In_le (u : UniverseLevel.t) v e :
+  UnivExprSet.In e u -> val v e <= val v u.
+Proof.
+  intro H. rewrite val_fold_right.
+  apply UniverseLevel.In_exprs_rev in H. destruct (UniverseLevel.exprs u); cbn in *.
+  clear -H. destruct H as [H|H].
+  - subst. induction (List.rev l); cbnr; lia.
+  - induction (List.rev l); cbn; invs H.
+    + u; lia.
+    + specialize (IHl0 H0). lia.
+Qed.
+
+Lemma val_In_max (u : UniverseLevel.t) v :
+  exists e, UnivExprSet.In e u /\ val v e = val v u.
+Proof.
+  eapply iff_ex. {
+    intro. eapply and_iff_compat_r. apply UniverseLevel.In_exprs_rev. }
+  rewrite val_fold_right. destruct (UniverseLevel.exprs u) as [e l]; cbn in *.
+  clear. induction (List.rev l); cbn.
+  - exists e. split; cbnr. left; reflexivity.
+  - destruct IHl0 as [e' [H1 H2]].
+    destruct (Nat.max_dec (val v a) (fold_right (fun e0 x0 => Nat.max (val v e0) x0)
+                                               (val v e) l0)) as [H|H];
+      rewrite H; clear H.
+    + exists a. split; cbnr. right. now constructor.
+    + rewrite <- H2. exists e'. split; cbnr.
+      destruct H1 as [H1|H1]; [now left|right]. now constructor 2.
+Qed.
+
+Lemma val_ge_caract (u : UniverseLevel.t) v k :
+  (forall e, UnivExprSet.In e u -> val v e <= k) <-> val v u <= k.
+Proof.
+  split.
+  - eapply imp_iff_compat_r. {
+      eapply iff_forall; intro. eapply imp_iff_compat_r.
+      apply UniverseLevel.In_exprs_rev. }
+    rewrite val_fold_right.
+    destruct (UniverseLevel.exprs u) as [e l]; cbn; clear.
+    induction (List.rev l); cbn.
+    + intros H. apply H. left; reflexivity.
+    + intros H.
+      destruct (Nat.max_dec (val v a) (fold_right (fun e0 x => Nat.max (val v e0) x)
+                                                 (val v e) l0)) as [H'|H'];
+        rewrite H'; clear H'.
+      * apply H. right. now constructor.
+      * apply IHl0. intros x [H0|H0]; apply H. now left.
+        right; now constructor 2.
+  - intros H e He. eapply val_In_le in He. etransitivity; eassumption.
+Qed.
+
+Lemma val_le_caract (u : UniverseLevel.t) v k :
+  (exists e, UnivExprSet.In e u /\ k <= val v e) <-> k <= val v u.
+Proof.
+  split.
+  - eapply imp_iff_compat_r. {
+      eapply iff_ex; intro. eapply and_iff_compat_r. apply UniverseLevel.In_exprs_rev. }
+    rewrite val_fold_right.
+    destruct (UniverseLevel.exprs u) as [e l]; cbn; clear.
+    induction (List.rev l); cbn.
+    + intros H. destruct H as [e' [[H1|H1] H2]].
+      * now subst.
+      * invs H1.
+    + intros [e' [[H1|H1] H2]].
+      * forward IHl0; [|lia]. exists e'. split; tas. left; assumption.
+      * invs H1.
+        -- u; lia.
+        -- forward IHl0; [|lia]. exists e'. split; tas. right; assumption.
+  - intros H. destruct (val_In_max u v) as [e [H1 H2]].
+    exists e. rewrite H2; split; assumption.
+Qed.
+
+
+
+Lemma val_caract (u : UniverseLevel.t) v k :
+  val v u = k
+  <-> (forall e, UnivExprSet.In e u -> val v e <= k)
+    /\ exists e, UnivExprSet.In e u /\ val v e = k.
+Proof.
+  split.
+  - intros <-; split.
+    + apply val_In_le.
+    + apply val_In_max.
+  - intros [H1 H2].
+    apply val_ge_caract in H1.
+    assert (k <= val v u); [clear H1|lia].
+    apply val_le_caract. destruct H2 as [e [H2 H2']].
+    exists e. split; tas. lia.
+Qed.
+
+Lemma val_add v e s
+  : val v (UniverseLevel.add e s) = Nat.max (val v e) (val v s).
+Proof.
+  apply val_caract. split.
+  - intros e' H. apply UnivExprSet.add_spec in H. destruct H as [H|H].
+    + subst. u; lia.
+    + eapply val_In_le with (v:=v) in H. lia.
+  - destruct (Nat.max_dec (val v e) (val v s)) as [H|H]; rewrite H; clear H.
+    + exists e. split; cbnr. apply UnivExprSetFact.add_1. reflexivity.
+    + destruct (val_In_max s v) as [e' [H1 H2]].
+      exists e'. split; tas. now apply UnivExprSetFact.add_2.
+Qed.
+
+Lemma val_sup v s1 s2 :
+  val v (UniverseLevel.sup s1 s2) = Nat.max (val v s1) (val v s2).
+Proof.
+  eapply val_caract. cbn. split.
+  - intros e' H. eapply UnivExprSet.union_spec in H. destruct H as [H|H].
+    + eapply val_In_le with (v:=v) in H. lia.
+    + eapply val_In_le with (v:=v) in H. lia.
+  - destruct (Nat.max_dec (val v s1) (val v s2)) as [H|H]; rewrite H; clear H.
+    + destruct (val_In_max s1 v) as [e' [H1 H2]].
+      exists e'. split; tas. apply UnivExprSet.union_spec. now left.
+    + destruct (val_In_max s2 v) as [e' [H1 H2]].
+      exists e'. split; tas. apply UnivExprSet.union_spec. now right.
+Qed.
+
+(* 
+Lemma val_zero_exprs v (l : Universe.t0) : 0 <= val v l.
+Proof.
+  rewrite val_fold_right.
+  destruct (Universe.exprs l) as [e u']; clear l; cbn.
+  induction (List.rev u'); simpl.
+  - destruct e as [npl_expr].
+    destruct npl_expr as [t b].
+    cbn.
+    assert (0 <= val v t) by apply Level.val_zero.
+    destruct b;lia.
+  - pose proof (UnivExpr.val_zero a v); lia.
+Qed. *)
+
+(** ** Extensionality lemmas on universe levels *)
+
+Lemma eq_univ (u v : UniverseLevel.t) :
+  u = v :> UnivExprSet.t -> u = v.
+Proof.
+  destruct u as [u1 u2], v as [v1 v2]; cbn. intros X; destruct X.
+  now rewrite (uip_bool _ _ u2 v2).
+Qed.
+
+Lemma eq_univ' (u v : UniverseLevel.t) :
+  UnivExprSet.Equal u v -> u = v.
+Proof.
+  intro H. now apply eq_univ, UnivExprSet.eq_leibniz.
+Qed.
+
+Lemma eq_univ'' (u v : UniverseLevel.t) :
+  UnivExprSet.elements u = UnivExprSet.elements v -> u = v.
+Proof.
+  intro H. apply eq_univ.
+  destruct u as [u1 u2], v as [v1 v2]; cbn in *; clear u2 v2.
+  destruct u1 as [u1 u2], v1 as [v1 v2]; cbn in *.
+  destruct H. now rewrite (uip_bool _ _ u2 v2).
+Qed.
+
+Lemma get_is_level_correct u l :
+  UniverseLevel.get_is_level u = Some l -> u = UniverseLevel.make l.
+Proof.
+  intro H.
+  destruct u.
+  cbn in *.
+  unfold UniverseLevel.make, UniverseLevel.make'.
+  unfold UniverseLevel.get_is_level in H.
+  destruct (UnivExprSet.elements _) as [|l0 L] eqn:Hu1; [discriminate|].
+  destruct l0, L; try discriminate.
+  * destruct n;inversion H;subst.
+    apply eq_univ'';unfold UnivExpr.make.
+    cbn. simpl in Hu1. rewrite Hu1. reflexivity.
+  * destruct e,n;inversion H;subst.
+Qed.
+
+Lemma univ_expr_eqb_true_iff (u v : UniverseLevel.t) :
+  UnivExprSet.equal u v <-> u = v.
+Proof.
+  split.
+  - intros.
+    apply eq_univ'. now apply UnivExprSet.equal_spec.
+  - intros ->. now apply UnivExprSet.equal_spec.
+Qed.
+
+Lemma eqb_true_iff u v :
+  UniverseLevel.eqb u v <-> u = v.
+Proof.
+  split. 2: intros ->; apply UniverseLevel.eqb_refl.
+  intro H.
+  destruct u,v;auto;try discriminate.
+  now apply univ_expr_eqb_true_iff.
+Qed.
+
+
+(** ** Lemmas on for_all *)
+
+Ltac proper := let H := fresh in try (intros ? ? H; destruct H; reflexivity).
+
+Lemma for_all_elements (P : UnivExpr.t -> bool) u :
+  UnivExprSet.for_all P u = forallb P (UnivExprSet.elements u).
+Proof.
+  apply UnivExprSetFact.for_all_b; proper.
+Qed.
+
+Lemma UnivExprSet_for_all_false f u :
+  UnivExprSet.for_all f u = false -> UnivExprSet.exists_ (negb ∘ f) u.
+Proof.
+  intro H. rewrite UnivExprSetFact.exists_b.
+  rewrite UnivExprSetFact.for_all_b in H.
+  all: try now intros x y [].
+  induction (UnivExprSet.elements u); cbn in *; [discriminate|].
+  apply andb_false_iff in H; apply orb_true_iff; destruct H as [H|H].
+  left; now rewrite H.
+  right; now rewrite IHl.
+Qed.
+
+Lemma UnivExprSet_For_all_exprs (P : UnivExpr.t -> Prop) (u : UniverseLevel.t)
+  : UnivExprSet.For_all P u
+    <-> P (UniverseLevel.exprs u).1 /\ Forall P (UniverseLevel.exprs u).2.
+Proof.
+  etransitivity.
+  - eapply iff_forall; intro e. eapply imp_iff_compat_r.
+    apply UniverseLevel.In_exprs.
+  - cbn; split.
+    + intro H. split. apply H. now left.
+      apply Forall_forall. intros x H0.  apply H; now right.
+    + intros [H1 H2] e [He|He]. subst e; tas.
+      eapply Forall_forall in H2; tea.
+Qed.
+
+
+
+(** ** Lemmas on sup of two universe levels *)
+
+Lemma sup_comm x1 x2 :
+  UniverseLevel.sup x1 x2 = UniverseLevel.sup x2 x1.
+Proof.
+  apply eq_univ'; simpl. unfold UnivExprSet.Equal.
+  intros H. rewrite !UnivExprSet.union_spec. intuition.
+Qed.
+
+
+(** ** Constraints on universe levels *)
+
+Module UnivConstraintType.
+  Inductive t_ : Set := Le (z : Z) | Eq.
+  Definition t := t_.
+  Definition eq : t -> t -> Prop := eq.
+  Definition eq_equiv : Equivalence eq := _.
+
+  Definition Le0 := Le 0.
+  Definition Lt := Le 1.
+
+  Inductive lt_ : t -> t -> Prop :=
+  | LeLe n m : (n < m)%Z -> lt_ (Le n) (Le m)
+  | LeEq n : lt_ (Le n) Eq.
+  Definition lt := lt_.
+
+  Lemma lt_strorder : StrictOrder lt.
+  Proof.
+    constructor.
+    - intros []; intro X; inversion X. lia.
+    - intros ? ? ? X Y; invs X; invs Y; constructor. lia.
+  Qed.
+
+  Lemma lt_compat : Proper (eq ==> eq ==> iff) lt.
+  Proof.
+    intros ? ? X ? ? Y; invs X; invs Y. reflexivity.
+  Qed.
+
+  Definition compare (x y : t) : comparison :=
+    match x, y with
+    | Le n, Le m => Z.compare n m
+    | Le _, Eq => Datatypes.Lt
+    | Eq, Eq => Datatypes.Eq
+    | Eq, _  => Datatypes.Gt
+    end.
+
+  Lemma compare_spec x y : CompareSpec (eq x y) (lt x y) (lt y x) (compare x y).
+  Proof.
+    destruct x, y; repeat constructor. simpl.
+    destruct (Z.compare_spec z z0); simpl; constructor.
+    subst; constructor. now constructor. now constructor.
+  Qed.
+
+  Lemma eq_dec x y : {eq x y} + {~ eq x y}.
+  Proof.
+    unfold eq. decide equality.
+    apply Z.eq_dec.
+  Qed.
+End UnivConstraintType.
+
+Module UnivConstraint.
+  Definition t : Set := Level.t * UnivConstraintType.t * Level.t.
+  Definition eq : t -> t -> Prop := eq.
+  Definition eq_equiv : Equivalence eq := _.
+
+  Definition make l1 ct l2 : t := (l1, ct, l2).
+
+  Inductive lt_ : t -> t -> Prop :=
+  | lt_Level2 l1 t l2 l2' : Level.lt l2 l2' -> lt_ (l1, t, l2) (l1, t, l2')
+  | lt_Cstr l1 t t' l2 l2' : UnivConstraintType.lt t t' -> lt_ (l1, t, l2) (l1, t', l2')
+  | lt_Level1 l1 l1' t t' l2 l2' : Level.lt l1 l1' -> lt_ (l1, t, l2) (l1', t', l2').
+  Definition lt := lt_.
+
+  Lemma lt_strorder : StrictOrder lt.
+  Proof.
+    constructor.
+    - intros []; intro X; inversion X; subst;
+        try (eapply Level.lt_strorder; eassumption).
+      eapply UnivConstraintType.lt_strorder; eassumption.
+    - intros ? ? ? X Y; invs X; invs Y; constructor; tea.
+      etransitivity; eassumption.
+      2: etransitivity; eassumption.
+      eapply UnivConstraintType.lt_strorder; eassumption.
+  Qed.
+
+  Lemma lt_compat : Proper (eq ==> eq ==> iff) lt.
+  Proof.
+    intros ? ? X ? ? Y; invs X; invs Y. reflexivity.
+  Qed.
+
+  Definition compare : t -> t -> comparison :=
+    fun '(l1, t, l2) '(l1', t', l2') =>
+      Pos.switch_Eq (Pos.switch_Eq (Level.compare l2 l2')
+                                   (UnivConstraintType.compare t t'))
+                    (Level.compare l1 l1').
+
+  Lemma compare_spec x y
+    : CompareSpec (eq x y) (lt x y) (lt y x) (compare x y).
+  Proof.
+    destruct x as [[l1 t] l2], y as [[l1' t'] l2']; cbn.
+    destruct (Level.compare_spec l1 l1'); cbn; repeat constructor; tas.
+    invs H.
+    destruct (UnivConstraintType.compare_spec t t'); cbn; repeat constructor; tas.
+    invs H.
+    destruct (Level.compare_spec l2 l2'); cbn; repeat constructor; tas.
+    invs H. reflexivity.
+  Qed.
+
+  Lemma eq_dec x y : {eq x y} + {~ eq x y}.
+  Proof.
+    unfold eq. repeat decide equality.
+  Defined.
+
+  Definition eq_leibniz (x y : t) : eq x y -> x = y := id.
+End UnivConstraint.
+
+Module UnivConstraintSet := MSetList.MakeWithLeibniz UnivConstraint.
+Module UnivConstraintSetFact := WFactsOn UnivConstraint UnivConstraintSet.
+Module UnivConstraintSetProp := WPropertiesOn UnivConstraint UnivConstraintSet.
+
+
+
